polymorphism/f_sub_diamond/examples_cell_opaque.v
@@ -1,0 +1,352 @@
+Require Export Arith.EqNat.
+Require Export Arith.Le.
+Require Import Coq.Arith.Arith.
+Require Import Coq.Bool.Bool.
+Require Import Coq.Program.Equality.
+Require Import Coq.Lists.List.
+Require Import Psatz.
+Require Import Coq.Arith.Compare_dec.
+Import ListNotations.
+
+Require Import vars.
+Require Import env.
+Require Import tactics.
+Require Import qualifiers.
+Require Import f_sub_diamond.
+Require Import examples_infra.
+
+Require Import NatSets.
+Require Import setfacts.
+Import NatSet.F.
+
+Import OpeningNotations.
+Local Open Scope opening.
+Import QualNotations.
+Local Open Scope qualifiers.
+
+(* This file demonstrates the general idea behind opaque typings for Church-encoded data types, which can be used when returning data that
+     closes over tracked local resources. We will exemplify the idea on the Cell[A] type with the usual System F encoding ∀C.(A => C) => C.  *)
+
+(* We make use of a few notations to make function and universal types more palatable: *)
+
+Notation " { a | b } ==> { c | d }"  := (TFun b d a c)
+(at level 10, format "'[' '[hv' '{' a  '/' '|'  b '}' ']' '/  '  '==>'  '[hv' '{' c  '/' '|'  d '}' ']' ']'").
+
+Notation "∀<:{ a | b }.{ c | d }"  := (TAll b d a c)
+(at level 10, format "'[' '[hv' '∀<:{' a  '/' '|'  b '}.{' ']' '/  '  '[hv' c  '/' '|'  d '}' ']' ']'").
+
+Notation "⊤" := TTop.
+
+(* shorthand if upper bound is the top type *)
+Notation "∀<:{ a }.{ c | d }" := (TAll a d ⊤ c) (at level 10, only parsing).
+(* even shorter *)
+Notation "∀.{ c | d }" := (TAll {♦} d ⊤ c) (at level 10, only parsing).
+
+Section DerivedSyntax.
+
+  (* Let bindings as macros for abstraction and application. Due to this encoding, the let-bound variable's
+     deBruijn index is #1, since the implicit function self reference is bound to #0.
+  *)
+  Definition val (t1 t2 : tm): tm := (tapp (tabs t2) t1).
+
+  (* the typing rule combines the tabs and t_app_fresh cases (we could also have a non-fresh version) *)
+  Lemma t_val_fresh : forall Γ φ df Σ t1 T1 q1 t2 T2 q2,
+    closed_tm 2 (length Γ) (length Σ) t2 ->
+    closed_ty 0 (‖Γ‖) (‖Σ‖) (TFun q1 q2 T1 T2) ->
+    closed_qual 2 (length Γ) (length Σ) q2 ->
+    closed_qual 0 (length Γ) (length Σ) df ->
+    has_type Γ φ Σ t1 T1 q1 ->
+    df ⊑ φ ->
+    (q2 <~ᵈ ∅ ; ∅) ⊑ φ ->
+    ♦∉ df ->
+    saturated Γ Σ df ->
+    saturated Γ Σ q1 ->
+    senv_saturated Σ (q2 <~ᵈ ∅ ; ∅) ->
+    not_free 0 T2 ->
+    (♦∈ q1 -> not_free 1 T2) ->
+    has_type (bind_tm(false, T1, (df ⋒ q1)) :: bind_tm(true, {T1 | df ⋒ q1} ==> {T2 | q2}, df):: Γ) (df ⊔ $!(S (length Γ)) ⊔ {♦}) Σ (open_tm' Γ t2) (open_ty' Γ T2) (openq' Γ q2) ->
+    has_type Γ φ Σ (val t1 t2) (T2 <~ᵀ TUnit ~ ∅ ; T1 ~ q1) (q2 <~ᵈ df ; q1).
+    intros. unfold val. specialize (has_type_closed H3). intuition.
+    eapply t_app_fresh with (d1':=q1) (df':=df); ccrush.
+    apply t_abs; ccrush. constructor; ccrush. inversion H0; subst. auto.
+    unfold_open in H12. simpl in H12.
+    eapply @weaken_flt with (φ:=df ⊔ $! (S (length Γ)) ⊔ {♦}); ccrush.
+    eapply has_type_filter; eauto.
+  Qed.
+
+  Lemma open_val : forall {k t t1 t2}, open_rec_tm k t (val t1 t2) = (val (open_rec_tm k t t1) (open_rec_tm (S (S k)) t t2)).
+    intros. unfold val. simpl. auto.
+  Qed.
+
+End DerivedSyntax.
+
+Section OpaqueCell.
+
+(*  Below is an _opaque_ cell type containing a datum reaching out-of-scope variables.
+
+    OCell[A] := p∀C^c<:⊤^∅. f(g(y:A^♦ -> C^y)^∅ -> C^f)^p
+
+    If we erase qualifiers, then we obtain the usual F(sub) encoding.
+
+    The intent is to be able to extract the (contextually fresh) datum of type A. As a first simplification, we do not make use
+    of the quantified c qualifier, and can thus set its bound to the empty (non-fresh) qualifier.
+
+    Using dependent function types, the extractor g(y:A^♦ -> C^y) specifies that the elimination's qualifier must come from the
+    stored datum itself, which to the extractor appears contextually fresh. Furthermore, given such a g function, OCell promises to return
+    a C^f, with some abstracted reachability set of the cell's computation f.
+
+    The technique we see at play here is a "self-reference chain" starting from the outer universal type p's self-reference, attached
+    to the inner function f, which then occurs in its codomain qualifier. That is to say, f reaches whatever p reaches, and we do not
+    need a "deep" occurrence of self-references in types, such as p∀C^c<:⊤^{}. f(g(y:A^♦ -> C^y)^∅ -> C^p) where p deeply occurs in
+    f's codomain.
+
+    Let's see this in action:
+
+    cell : (p∀C^c<:⊤^{}. f(g(y:A^♦ -> C^y)^∅ -> C^f)^p)^{cell}  ⊣ cell : OCell[A]^{♦}
+
+    cell[A^∅] : f(g(y:A^♦ -> A^y)^∅ -> A^f)^{cell} // By type application: p ↦ {cell}
+
+    let id: g(y:A^♦ -> A^y)^∅ = x => x // The extractor (identity) can be assigned this type
+
+    cell[A^∅](id) : A^{cell} // By function application: f ↦ {cell}
+
+    That is, we have propagated the name of the cell to the result's qualifier. And that is all we can really know
+    about an opaque data type.
+
+    In the remainder of this file, we fully mechanize opaque cells end to end in our calculus.
+*)
+
+  (* OCell[A] := p∀C^c<:⊤^{}. f(g(y:A^♦ -> C^y)^∅ -> C^f)^p
+     Note: the number attached to the element type parameter indicates by how much it must be incremented if it is a deBruijn index.
+    *)
+  Example TOCell A2 := (∀<:{ ∅ }.{ { { A2 | {♦} } ==> { #3 | #!1 } | ∅ } ==> { #3 | #!0 } | #!0 }).
+
+  (* Cell introduction: ΛA.λx.ΛC.λf.f(x) *)
+  Example cell_mk := (ttabs (tabs (ttabs (tabs (tapp #1 #5))))).
+  (* Cell elimination: ΛA.λc.c[A](id) *)
+  Example cell_get := (ttabs (tabs (tapp (ttapp #1) (tabs #1)))).
+
+  (* Cell introduction typing
+     cell_mk : z[A^a<:⊤^♦] => (g(x: A^a) => (p[C^c<:⊤^{}] => f(h(y:A^♦ => C^y)^∅ => C^f)^p)^x,g)^a *)
+  Example t_cell_chained2_abs_ :
+    has_type [] ∅ [] cell_mk (∀.{ {#1 | #!1} ==> (*A:#3 x:#1 *) {TOCell #5 | #!0 ⊔ #!1 } | #!1 }) ∅.
+    unfold cell_mk.
+    apply t_tabs; ccrush. unfold TOCell. ccrush.
+    apply t_abs; ccrush.
+    (* g abstraction: *)
+    (* x,a <: x,g *)
+    eapply t_sub with (d1:=$!3 ⊔ $!1).
+    2 : {
+        eapply stp_refl; try solve [ccrush].
+        replace (qset false (union (singleton 2) (singleton 3)) {}N {}N) with ($!3 ⊔ $!2); try solve [ccrush].
+        apply qs_cong; try solve [ccrush].
+        apply qs_trans with (d2:=$!1 ⊔ $!2).
+        apply qs_sq; ccrush. eapply qs_self; ccrush.
+    } 2,3 : ccrush.
+    apply t_tabs; ccrush.
+    (* p abstraction: *)
+    (* x,a <: p  *)
+    eapply t_sub with (d1:=$!3 ⊔ $!1).
+    2: {
+        eapply stp_refl; try solve [ccrush].
+        apply qs_trans with (d2:=($!3 ⊔ $!1) ⊔ $!4).
+        apply qs_sq; ccrush. eapply qs_self_all; ccrush.
+    } 2,3 : ccrush.
+    apply t_abs; ccrush.
+    (* f abstraction: *)
+    (* x <: x,a <: f*)
+    apply t_sub with (T1:=$5) (d1:=$!3).
+    2: {
+        apply stp_refl; try solve [ccrush].
+        apply qs_trans with (d2:=($!3 ⊔ $!1) ⊔ $!6).
+        apply qs_sq; ccrush. eapply qs_self; ccrush.
+    } 2-3: ccrush.
+    change_qual (openq $!7 $!3 #!1).
+    change_type (open_ty TUnit ∅ $1 $!3 $5).
+    apply t_app_fresh with (df':=$!7) (d1':=$♦3 ⊔ $♦1); try solve [ccrush].
+    * dom_equals ({♦}). cleanup.
+      eapply t_var; ccrush. simpl. repeat f_equal; try fnsetdec. apply NatSet.eq_if_Equal.
+      split; try fnsetdec. rewrite empty_union_right. intros.
+      apply NatSetFacts.inter_iff in H. intuition.
+      apply union_1 in H1. intuition. all: apply NatSetProperties.FM.singleton_iff in H0, H; subst; discriminate.
+    * eapply t_var; ccrush.
+    * constructor; auto. unfold tenv_saturated. intros.
+        apply qmem_lub_or_commute in H. intuition.
+        simpl in H0; apply NatSetFacts.singleton_iff in H0; subst.
+        econstructor; ccrush. simpl in H0; apply NatSetFacts.singleton_iff in H0; subst.
+        eapply sat_tvar. ccrush. all : ccrush.
+  Qed.
+
+  (* generalize to all contexts *)
+  Example t_cell_chained2_abs : forall {Γ φ Σ}, closed_qual 0 (‖Γ‖) (‖Σ‖) φ ->
+    has_type Γ φ Σ cell_mk (∀.{ {#1 | #!1} ==> (*A:#3 x:#1 *) {TOCell #5 | #!0 ⊔ #!1 } | #!1 }) ∅.
+    intros. eapply weaken'. eapply weaken_store. apply t_cell_chained2_abs_. all : auto.
+  Qed.
+
+  (* The identity is a compatible extractor
+     id : (y:A^♦ => A^y)^∅ *)
+  Example id_elim2 : forall Γ φ Σ A,
+    closed_qual 0 (‖ Γ ‖) (‖ Σ ‖) φ -> closed_ty 0 (‖ Γ ‖) (‖ Σ ‖) A ->
+    has_type Γ φ Σ (tabs #1) ({ A | {♦} } ==> {A | #!1 }) ∅.
+    intros.
+    apply t_abs; ccrush.
+    eapply t_var; ccrush.
+  Qed.
+
+  (* Cell elimination typing
+     cell_get: (f[A^a <: ⊤^♦] => (OCell[A]^{a} => A^a)^a)^∅ *)
+  Example t_cell_get_abs_ :
+    has_type [] ∅ [] cell_get (∀.{ {TOCell #3 | #!1 } ==> { #3 | #!3 } | #!1 }) ∅.
+    unfold cell_get.
+    apply t_tabs; ccrush. unfold TOCell. ccrush.
+    apply t_abs; ccrush.
+    change_qual (openq $!1 ∅ (#!0)).
+    change_type (open_ty TUnit ∅ ({$ 1 | {♦}} ==> {$1 | #!1}) ∅ $1).
+    apply t_app; ccrush.
+    * change_qual (openq $!1 ∅ (#!0)).
+      change_type (open_ty TUnit ∅ $1 ∅ ({{$ 1 | {♦}} ==> {# 3 | #! 1} | ∅} ==> {# 3 | #!0 })).
+      apply t_tapp; ccrush. (* it's sufficient to instantiate with precise, non-fresh bound *)
+      eapply t_sub. eapply t_var; ccrush. apply s_all; ccrush.
+      eapply qs_qvar; ccrush. apply stp_refl; ccrush. apply qs_sq; ccrush.
+      all : ccrush.
+    * apply id_elim2; ccrush.
+  Qed.
+
+  (* generalize to all contexts *)
+  Example t_cell_get_abs : forall {Γ φ Σ}, closed_qual 0 (‖Γ‖) (‖Σ‖) φ ->
+    has_type Γ φ Σ cell_get (∀.{ {TOCell #3 | #!1 } ==> { #3 | #!3 } | #!1 }) ∅.
+    intros. eapply weaken'. eapply weaken_store. apply t_cell_get_abs_. all : auto.
+  Qed.
+
+End OpaqueCell.
+
+Section OpaqueCellUse.
+
+  (* A concrete usage example *)
+
+  Context (Σ := [(TUnit, ∅); ({ TUnit | ∅} ==> {TUnit | ∅}, ∅)])
+          (φ := ({♦} ⊔ &!0 ⊔ &!1)).
+
+  (* cell_get[_](cell_mk[_](&1)) *)
+  Example get_mk_cell := (tapp (ttapp cell_get) (tapp (ttapp cell_mk) &1)).
+
+  Lemma sat_loc_1: saturated [] Σ &!1.
+    unfold Σ. constructor; eauto.
+    unfold senv_saturated. intros. simpl in H; apply NatSetFacts.singleton_iff in H; subst.
+    apply sat_loc with (U:=TUnit) (q':=∅); ccrush.
+    Unshelve. auto.
+  Qed.
+
+  (* Type instantiation of the extractor used in this example *)
+  Example t_cell_get_abs_inst: has_type [] φ Σ (ttapp cell_get) ({TOCell (TRef ∅ TUnit) | &!1 } ==> { (TRef ∅ TUnit) | &!1 }) &!1.
+    change_qual (openq ∅ &!1 #!1).
+    change_type (open_ty TUnit ∅ (TRef ∅ TUnit) &!1 ({TOCell #3 | #!1 } ==> { #3 | #!3 })).
+    apply t_tapp_fresh with (d1':=&!1) (df':=∅) ; try solve [unfold TOCell; ccrush].
+    eapply t_sub. eapply t_cell_get_abs; ccrush.
+    apply s_all. 1-4 : unfold TOCell; ccrush.
+    cleanup. apply stp_refl; ccrush. apply qs_sq; ccrush.
+    all : ccrush. all: eauto using sat_loc_1.
+  Qed.
+
+  (* Type instantiaion of the introduction used in this example *)
+  Example t_cell_mk_abs_inst: has_type [] φ Σ (ttapp cell_mk) ({(TRef ∅ TUnit) | &!1 } ==> {TOCell (TRef ∅ TUnit) | #!0 ⊔ #!1 }) &!1.
+    change_qual (openq ∅ &!1 #!1).
+    change_type (open_ty TUnit ∅ (TRef ∅ TUnit) &!1 ({#1 | #!1} ==> {TOCell #5 | #!0 ⊔ #!1 })).
+    apply t_tapp_fresh with (d1':=&!1) (df':=∅) ; try solve [unfold TOCell; ccrush].
+    eapply t_sub. eapply t_cell_chained2_abs; ccrush.
+    apply s_all. 1-4 : unfold TOCell; ccrush.
+    cleanup. apply stp_refl; ccrush. apply qs_sq; ccrush.
+    all : ccrush. all: eauto using sat_loc_1.
+  Qed.
+
+  (* Typing the example *)
+  Example t_get_mk_cell_abs : has_type [] φ Σ get_mk_cell (TRef ∅ TUnit) &!1.
+    unfold get_mk_cell.
+    change_qual (openq &!1 &!1 &!1).
+    change_type (open_ty TUnit ∅ (TOCell (TRef ∅ TUnit)) &!1 (TRef ∅ TUnit)).
+    apply t_app; ccrush. 3 : eauto using sat_loc_1.
+    * apply t_cell_get_abs_inst.
+    * change_qual (openq &!1 &!1 (#!0 ⊔ #!1)).
+      change_type (open_ty TUnit ∅ (TRef ∅ TUnit) &!1 (TOCell (TRef ∅ TUnit))).
+      apply t_app; try solve [ccrush].
+      - apply t_cell_mk_abs_inst.
+      - change_qual (∅ ⊔ &!1). apply t_loc; ccrush.
+  Qed.
+
+End OpaqueCellUse.
+
+Section OpaqueCellEndToEnd.
+
+  (* Another example, mirroring the "counter" (Fig. 1 in the paper), just on a single cell *)
+
+  (* Thunk type *)
+  Example TThunk := ({TUnit | ∅ } ==> {TUnit | ∅}).
+
+  (* A closure analogous to the counter:
+
+    def cell_closure() =
+      let x = new Ref()
+      cell_mk(() => x:=!x)
+  *)
+  Example cell_closure := (tabs (val (tref tunit)
+                                     (tapp (ttapp cell_mk) (tabs (tassign #3 (tderef #3)))))).
+
+  (* Usage:
+
+     let cell = cell_closure() // : OCell[TThunk]^{cell}
+        cell_get(cell)         // : TThunk^{cell} within the let body, and TThunk^{♦} for the entire expression
+  *)
+  Example cell_closure_use := (val (tapp cell_closure tunit) (tapp (ttapp cell_get) #1)).
+
+  (* cell_closure : Unit => OCell[Thunk]^{♦} *)
+  Example t_cell_closure : has_type [] ∅ [] cell_closure ({TUnit | ∅ } ==> { (TOCell TThunk) | {♦} }) ∅.
+    unfold cell_closure. unfold TOCell.
+    apply t_abs; try solve [ccrush]. unfold TThunk; ccrush.
+    unfold_open. repeat rewrite open_val. cleanup. fold cell_mk. fold TThunk.
+    change_qual (openq ∅ {♦} #!1).
+    change_type ((∀<:{⊤ | ∅ }.{ {{ TThunk | {♦}} ==> {# 3 | #!1 } | ∅} ==> {# 3 | #!0 } | #!0}) <~ᵀ TUnit ~ ∅; (TRef ∅ TUnit) ~ {♦}).
+    apply t_val_fresh; ccrush. unfold TThunk. ccrush.
+    * change_qual (∅ ⊔ {♦}). apply t_ref; ccrush. apply t_base; ccrush.
+    * fold cell_mk. fold TThunk.
+      change_qual (openq $!3 $!3 (#!0 ⊔ #!1)).
+      change_type ((∀<:{⊤ | ∅}.{ {{TThunk | {♦}} ==> {# 3 | #! 1} | ∅} ==> {# 3 | #! 0} | #! 0}) <~ᵀ TUnit ~ ∅; TThunk ~  $! 3).
+      apply t_app; try solve [ccrush].
+      + change_qual (openq ∅ $!3 #!1).
+        change_type (({#1 | #!1} ==> {∀<:{⊤ | ∅}.{ {{#5 | {♦}} ==> {# 3 | #! 1} | ∅} ==> {# 3 | #! 0} | #! 0} | #! 0 ⊔ #! 1}) <~ᵀ TUnit ~ ∅; TThunk ~ $! 3).
+        eapply t_tapp_fresh with (d1':=$♦3) (df':=∅); ccrush. 2: unfold TThunk; ccrush.
+        eapply t_sub. 3,4: ccrush.
+        ** eapply t_cell_chained2_abs; ccrush.
+        ** unfold TOCell. cleanup. eapply s_all. 1-4 : unfold TOCell; unfold TThunk; ccrush. cleanup.
+           apply stp_refl; ccrush. apply qs_sq; ccrush.
+      + apply t_abs; ccrush.
+        eapply t_assign.
+        ** eapply t_var; ccrush.
+        ** eapply t_deref. eapply t_var; ccrush. all: ccrush.
+        ** auto.
+  Qed.
+
+  (* cell_closure_use : TThunk^{♦} *)
+  Example t_cell_closure_use : has_type [] {♦} [] cell_closure_use TThunk {♦}.
+    unfold cell_closure_use.
+    change_qual (openq ∅ {♦} #!1).
+    change_type (open_ty TUnit ∅ (TOCell TThunk) {♦} TThunk).
+    apply t_val_fresh; try solve [ccrush]. 1 : unfold TOCell; unfold TThunk; ccrush.
+    * change_qual (openq ∅ ∅ {♦}).
+      dep_app (∅) (∅).
+      apply t_app; try solve [ccrush].
+      cleanup. eapply weaken_flt. apply t_cell_closure. all: ccrush.
+    * cleanup. fold cell_get. fold TThunk.
+      change_qual (openq $!1 $!1 $!1).
+      change_type (open_ty TUnit ∅ (TOCell TThunk) $!1 TThunk).
+      apply t_app; ccrush.
+      + change_qual (openq ∅ $!1 #!1).
+        change_type (open_ty TUnit ∅ TThunk $!1 ({TOCell #3 | #!1 } ==> {#3 | #!3})).
+        apply t_tapp_fresh with (d1':=$♦1) (df':=∅); ccrush. 2: unfold TThunk; ccrush.
+        eapply t_sub. 3,4: ccrush.
+        ** eapply t_cell_get_abs; ccrush.
+        ** unfold TOCell. cleanup. apply s_all. 1-4: unfold TThunk; ccrush. cleanup.
+           apply stp_refl; ccrush. apply qs_sq; ccrush.
+      + eapply t_var; ccrush. unfold TOCell. unfold TThunk. ccrush.
+  Qed.
+
+End OpaqueCellEndToEnd.
