polymorphism/f_sub_diamond/examples_pairs.v
@@ -1,0 +1,1246 @@
+Require Export Arith.EqNat.
+Require Export Arith.Le.
+Require Import Coq.Arith.Arith.
+Require Import Coq.Bool.Bool.
+Require Import Coq.Program.Equality.
+Require Import Coq.Lists.List.
+Require Import Psatz.
+Require Import Coq.Arith.Compare_dec.
+Import ListNotations.
+
+Require Import vars.
+Require Import env.
+Require Import tactics.
+Require Import qualifiers.
+Require Import f_sub_diamond.
+Require Import examples_infra.
+
+Require Import NatSets.
+Require Import setfacts.
+Import NatSet.F.
+
+Import OpeningNotations.
+Local Open Scope opening.
+Import QualNotations.
+Local Open Scope qualifiers.
+
+(* This file demonstrates the pair data type based on Church encodings. We encode both _transparent_ and _opaque_ pairs.
+   The former kind is used if the stored data reaches known resources in the context, whereas the latter can be used to
+   return data capturing out-of-scope resources.
+
+   As a warmup for opaque Church pairs, we recommend reviewing examples_cell_opaque.v first. *)
+
+(* We make use of a few notations to make function and universal types more palatable: *)
+
+Notation " { a | b } ==> { c | d }"  := (TFun b d a c)
+(at level 10, format "'[' '[hv' '{' a  '/' '|'  b '}' ']' '/  '  '==>'  '[hv' '{' c  '/' '|'  d '}' ']' ']'").
+
+Notation "∀<:{ a | b }.{ c | d }"  := (TAll b d a c)
+(at level 10, format "'[' '[hv' '∀<:{' a  '/' '|'  b '}.{' ']' '/  '  '[hv' c  '/' '|'  d '}' ']' ']'").
+
+Notation "⊤" := TTop.
+
+(* shorthand if upper bound is the top type *)
+Notation "∀<:{ a }.{ c | d }" := (TAll a d ⊤ c) (at level 10, only parsing).
+(* even shorter *)
+Notation "∀.{ c | d }" := (TAll {♦} d ⊤ c) (at level 10, only parsing).
+
+Section DerivedSyntax.
+
+  (* Let bindings as macros for abstraction and application. Due to this encoding, the let-bound variable's
+     deBruijn index is #1, since the implicit function self reference is bound to #0.
+  *)
+  Definition tlet (t1 t2 : tm): tm := (tapp (tabs t2) t1).
+
+  (* the typing rule combines the tabs and t_app_fresh cases (we could also have a non-fresh version) *)
+  Lemma t_let_fresh : forall Γ φ df df' Σ t1 T1 q1 q1' t2 T2 q2,
+    closed_tm 2 (length Γ) (length Σ) t2 ->
+    closed_ty 0 (‖Γ‖) (‖Σ‖) (TFun q1 q2 T1 T2) ->
+    closed_qual 2 (length Γ) (length Σ) q2 ->
+    closed_qual 0 (length Γ) (length Σ) df ->
+    has_type Γ φ Σ t1 T1 q1 ->
+    q1 ⊑ q1' ->
+    df ⊑ df' ->
+    q1' ⊑ φ ->
+    df' ⊑ φ ->
+    df ⊑ φ ->
+    (q2 <~ᵈ ∅ ; ∅) ⊑ φ ->
+    ♦∉ df ->
+    senv_saturated Σ df ->
+    saturated Γ Σ df' ->
+    saturated Γ Σ q1' ->
+    senv_saturated Σ (q2 <~ᵈ ∅ ; ∅) ->
+    not_free 0 T2 ->
+    (♦∈ q1 -> not_free 1 T2) ->
+    has_type (bind_tm(false, T1, (df' ⋒ q1')) :: bind_tm(true, {T1 | df' ⋒ q1'} ==> {T2 | q2}, df):: Γ) (df ⊔ $!(S (length Γ)) ⊔ {♦}) Σ (open_tm' Γ t2) (open_ty' Γ T2) (openq' Γ q2) ->
+    has_type Γ φ Σ (tlet t1 t2) (T2 <~ᵀ TUnit ~ ∅ ; T1 ~ q1) (q2 <~ᵈ df ; q1).
+  Proof.
+    intros. unfold tlet. specialize (has_type_closed H3). intuition.
+    eapply t_app_fresh with (d1':=q1') (df':=df'); ccrush.
+    apply t_abs; ccrush. constructor; ccrush. inversion H0; subst. auto.
+    unfold_open in H17. simpl in H17.
+    eapply @weaken_flt with (φ:=df ⊔ $! (S (length Γ)) ⊔ {♦}); ccrush.
+  Qed.
+
+  Lemma open_tlet : forall {k t t1 t2}, open_rec_tm k t (tlet t1 t2) = (tlet (open_rec_tm k t t1) (open_rec_tm (S (S k)) t t2)).
+  Proof.
+    intros. unfold tlet. simpl. auto.
+  Qed.
+
+End DerivedSyntax.
+
+
+(* Church pairs *)
+(* Pair introduction: ΛA.ΛB.λx:A.λy:B.ΛC.λf.f x y *)
+Example pair_mk := (ttabs (ttabs (tabs (tabs (ttabs (tabs (tapp (tapp #1 #7) #5))))))).
+(* Pair destructors *)
+(* fst = ΛA.ΛB.λp.p[A](x => y => x) *)
+Example fst := (ttabs (ttabs (tabs (tapp (ttapp #1) (tabs (tabs #3)))))).
+(* snd = ΛA.ΛB.λp.p[B](x => y => y)*)
+Example snd := (ttabs (ttabs (tabs (tapp (ttapp #1) (tabs (tabs #1)))))).
+
+Section PairTransparent.
+
+  (* We first cover the _transparent_ pairs, which support precise data extraction thanks to type-and-qualifier polymorphism (paper Section 2.4).
+
+     Pair[A^a,B^b] := ∀C^c<:⊤^a,b♦. (((x : A^a) -> ((y : B^b) -> C^c)^x)^{} -> C^c)^c,a,b
+
+     Ignoring qualifiers, this type corresponds to the standard Church encoding in System F(sub).
+
+     As explained in the paper, type-and-qualifier abstraction permits precise eliminations:
+
+     p : Pair[A^a, B^b]^{a,b}
+     p[A^a] : (((x : A^a) -> ((y : B^b) -> A^a)^x)^{} -> A^a)^a,b
+     p[B^b] : (((x : A^a) -> ((y : B^b) -> B^b)^x)^{} -> B^b)^a,b
+
+     It is important to permit the bound C^c<:⊤^a,b♦ so that the instantiation for c can overlap with a and b. Otherwise, it is impossible
+     to instantiate the pair's elimination to A^a and B^b respectively.
+  *)
+
+  Variables (Γ : tenv) (φ : qual) (Σ : senv).
+  Context (phiwf : closed_qual 0 (‖Γ‖) (‖Σ‖) φ).
+
+  (* Pair[A^a,B^b] := ∀C^c<:⊤^a,b♦. (((x : A^a) -> ((y : B^b) -> C^c)^x)^{} -> C^c)^c,a,b
+     Note: the number attached to each parameter indicates by how much it must be incremented if it is a deBruijn index.
+    *)
+  Example TPair A2 a0 a2 B4 b0 b2 b4 := ∀<:{ a0 ⊔ b0 ⊔ {♦} }.{ {{A2 | a2} ==> {{B4 | b4} ==> { #5 | #!5 } | #!1} | ∅ } ==> {#3 | #!3} | #!1 ⊔ a2 ⊔ b2 }.
+
+  (* The transparent pair introduction's type:
+     pair_mk: (∀A^a<:⊤^♦. (∀B^b<:⊤^a,♦. ( (x : A^a) -> ((y : B^b) -> (Pair[A^x,B^y])^x,y)^x))^a,b)^∅
+     Again, overlap is important here. We generally want to allow overlapping pair components, which is why the bound for b mentions a.
+     If we didn't include this, then we could construct strictly disjoint pairs.
+   *)
+  Example t_pair1_ :
+    has_type [] ∅ [] pair_mk (∀.{ ∀<:{ #♦1 }.{ {#3 | #!3} ==> {{#3 | #!3 } ==> (*A: #7, B: #5, x:#3, y:#1*) {TPair #9 #!3 #!5 #9 #!1 #!3 #!5 | (#!3 ⊔ #!1) } | #!1 }  | #!1 ⊔ #!3 } | #!1 }) ∅.
+    unfold pair_mk.
+    apply t_tabs; ccrush. unfold TPair. ccrush. (* 0/1*)
+    apply t_tabs; ccrush. (* 2/3 *)
+    apply t_abs; ccrush. (* 4/5 *)
+    apply t_abs; ccrush. (* 6/7 *)
+    apply t_tabs; ccrush. (* 8/9 *)
+    apply t_abs; ccrush.  (* 10/11 *)
+    change_qual (openq $!5 $!7 $!9).
+    change_type (open_ty TUnit (∅) ($3) $!7 $9).
+    apply t_app; ccrush.
+    * change_qual (openq $!11 $!5 #!1).
+      change_type (open_ty TUnit (∅) $1 $!5 ({$ 3 | $! 7} ==> {$ 9 | $! 9})).
+      apply t_app; ccrush.
+      + eapply t_var; ccrush.
+      + eapply t_sub. eapply t_var; ccrush.
+        apply stp_refl; ccrush. apply qs_sq; ccrush. all : ccrush.
+    * eapply t_var; ccrush.
+  Qed.
+
+  (* generalize to all contexts *)
+  Example t_pair1 :
+    has_type Γ φ Σ pair_mk (∀.{ ∀<:{ #♦1 }.{ {#3 | #!3} ==> {{#3 | #!3 } ==> (*A: #7, B: #5, x:#3, y:#1*) {TPair #9 #!3 #!5 #9 #!1 #!3 #!5 | (#!3 ⊔ #!1) } | #!1 }  | #!1 ⊔ #!3 } | #!1 }) ∅.
+    eapply weaken'. eapply weaken_store. apply t_pair1_. all : auto.
+  Qed.
+
+  (* Assert that the projection functions are compatible with each pair type (and extract the precise component qualifier!) *)
+  (* fst : (∀A^a<:⊤^♦. (∀B^b<:⊤^a,♦. (Pair1[A^a,B^b]^{a,b,♦} -> A^a)^a,b)^a)^∅ *)
+  Example t_fst1_ :
+    has_type [] ∅ [] fst (∀.{ ∀<:{ #♦1 }.{ {TPair #5 #!3 #!5 #5 #!1 #!3 #!5 | #!1 ⊔ #!3 ⊔ {♦} } ==> { #5 | #!5 } | #!1 ⊔ #!3 } | #!1 }) ∅.
+    unfold fst.
+    apply t_tabs; ccrush. unfold TPair. ccrush.
+    apply t_tabs; ccrush.
+    apply t_abs; ccrush.
+    change_qual (openq (qset false (union (singleton 1) (singleton 3)) {}N {}N) (∅) $!1).
+    change_type (open_ty TUnit (∅) ({$ 1 | $! 1} ==> {{$ 3 | $! 3} ==> {$1 | $! 1} | #!1}) (∅) $1).
+    apply t_app; ccrush.
+    * change_qual (openq ($!5) $!1 (qset false (union (singleton 1) (singleton 3)) (singleton 1) {}N)).
+      change_type (open_ty TUnit ∅ $1 $!1 ({{$ 1 | $! 1} ==> {{$ 3 | $! 3} ==> {# 5 | #! 5} | #! 1} | ∅} ==> {# 3 | #! 3})).
+      eapply t_tapp_fresh with (d1':=$♦1) (df':=$♦1 ⊔ $♦3 ⊔ $♦5) ; try solve [ccrush].
+      dom_equals ($♦ 1).
+      eapply t_sub.
+      eapply t_var; ccrush.
+      apply s_all. ccrush. ccrush.
+      apply qs_sq; ccrush.
+      eapply s_tvar_trans; ccrush. cleanup. apply stp_refl; ccrush. apply qs_sq; ccrush.
+      simpl. intuition. ccrush. auto.
+      ccrush. econstructor. unfold tenv_saturated. intros.
+      simpl in H. apply union_1 in H. destruct H. apply NatSetFacts.singleton_iff in H. subst.
+      try solve [eapply sat_tvar; ccrush].
+      apply union_1 in H; destruct H; apply NatSetFacts.singleton_iff in H; subst;
+        try solve [eapply sat_tvar; ccrush].
+      try solve [eapply sat_var; ccrush].
+      ccrush.
+    * eapply t_sub with (T1 := {$ 1 | $! 1} ==> {{$ 3 | $! 3} ==> { $1 | #!3 } | #! 1}) (d1:= ∅). 3,4: ccrush.
+      - apply t_abs; ccrush.
+        apply t_abs; ccrush.
+        eapply t_var; ccrush.
+      - apply s_fun; ccrush.
+        apply stp_refl; ccrush. apply qs_sq; ccrush.
+        apply s_fun; ccrush. apply qs_sq; ccrush.
+        apply stp_refl; ccrush. apply qs_sq; ccrush.
+        apply stp_refl; ccrush. eapply qs_qvar; ccrush.
+  Qed.
+
+  Example t_fst1 :
+    has_type Γ φ Σ fst (∀.{ ∀<:{ #♦1 }.{ {TPair #5 #!3 #!5 #5 #!1 #!3 #!5 | #!1 ⊔ #!3 ⊔ {♦} } ==> { #5 | #!5 } | #!1 ⊔ #!3 } | #!1 }) ∅.
+    eapply weaken'. eapply weaken_store. apply t_fst1_. all : auto.
+  Qed.
+
+  (* snd : (∀A^a<:⊤^♦. (∀B^b<:⊤^{a,♦}. (Pair1[A^a,B^b]^{a,b,♦} -> B^b)^a,b)^a)^∅ *)
+  Example t_snd1_ :
+    has_type [] ∅ [] snd (∀.{  ∀<:{ #♦1 }.{ {TPair #5 #!3 #!5 #5 #!1 #!3 #!5 | #!1 ⊔ #!3 ⊔ {♦} } ==> { #3 | #!3 } | #!1 ⊔ #!3 } | #!1 }) ∅.
+    unfold snd.
+    apply t_tabs; ccrush. unfold TPair. ccrush.
+    apply t_tabs; ccrush.
+    apply t_abs; ccrush.
+    change_qual (openq (qset false (union (singleton 1) (singleton 3)) {}N {}N) (∅) $!3).
+    change_type (open_ty TUnit (∅) ({$ 1 | $! 1} ==> {{$ 3 | $! 3} ==> {$3 | $! 3} | #!1}) (∅) $3).
+    apply t_app; ccrush.
+    * change_qual (openq ($!5) $!3 (qset false (union (singleton 1) (singleton 3)) (singleton 1) {}N)).
+      change_type (open_ty TUnit ∅ $3 $!3 ({{$ 1 | $! 1} ==> {{$ 3 | $! 3} ==> {# 5 | #! 5} | #! 1} | ∅} ==> {# 3 | #! 3})).
+      eapply t_tapp_fresh with (d1':=$♦1 ⊔ $♦3) (df':=$♦1 ⊔ $♦3 ⊔ $♦5) ; try solve [ccrush].
+      dom_equals ($♦1 ⊔ $♦3).
+      eapply t_sub.
+      eapply t_var; ccrush.
+      apply s_all. ccrush. ccrush.
+      apply qs_sq; ccrush.
+      eapply s_tvar_trans; ccrush. cleanup. apply stp_refl; ccrush. apply qs_sq; ccrush.
+      simpl. intuition. ccrush. auto.
+      econstructor; ccrush; unfold tenv_saturated; intros;
+      simpl in H; apply union_1 in H; destruct H; apply NatSetFacts.singleton_iff in H; subst;
+        try solve [eapply sat_tvar; ccrush].
+      econstructor; ccrush; unfold tenv_saturated; intros;
+      simpl in H; apply union_1 in H; destruct H. apply NatSetFacts.singleton_iff in H; subst;
+        try solve [eapply sat_tvar; ccrush].
+      apply union_1 in H. destruct H; apply NatSetFacts.singleton_iff in H; subst;
+        try solve [eapply sat_tvar; ccrush]; try solve [eapply sat_var; ccrush].
+    * eapply t_sub with (T1 := {$ 1 | $! 1} ==> {{$ 3 | $! 3} ==> { $3 | #!1 } | #! 1}) (d1:= ∅). 3,4: ccrush.
+      - apply t_abs; ccrush.
+        apply t_abs; ccrush.
+        eapply t_var; ccrush.
+      - apply s_fun; ccrush.
+        apply stp_refl; ccrush. apply qs_sq; ccrush.
+        apply s_fun; ccrush. apply qs_sq; ccrush.
+        apply stp_refl; ccrush. apply qs_sq; ccrush.
+        apply stp_refl; ccrush. eapply qs_qvar; ccrush.
+  Qed.
+
+  Example t_snd1 :
+    has_type Γ φ Σ snd (∀.{  ∀<:{ #♦1 }.{ {TPair #5 #!3 #!5 #5 #!1 #!3 #!5 | #!1 ⊔ #!3 ⊔ {♦} } ==> { #3 | #!3 } | #!1 ⊔ #!3 } | #!1 }) ∅.
+    eapply weaken'. eapply weaken_store. apply t_snd1_. all : auto.
+  Qed.
+
+End PairTransparent.
+
+Section PairTransparentUse.
+
+  (* a usage example over some arbitrary component types *)
+
+  Variables (Γ : tenv) (φ : qual) (Σ : senv).
+  Context (phiwf : closed_qual 0 (‖Γ‖) (‖Σ‖) φ).
+
+  Context (A B : ty)
+          (a b : qual)
+          (nf_a  : ♦∉ a)
+          (nf_b  : ♦∉ b)
+          (sat_a : saturated Γ Σ (a ⊔ {♦}))
+          (sat_b : saturated Γ Σ (b ⊔ {♦}))
+          (cl_a : closed_qual 0 (length Γ) (length Σ) a)
+          (cl_b : closed_qual 0 (length Γ) (length Σ) b)
+          (cl_A : closed_ty 0 (length Γ) (length Σ) A)
+          (cl_B : closed_ty 0 (length Γ) (length Σ) B)
+          (a_obs : a ⊑ φ)
+          (b_obs : b ⊑ φ)
+          (phi_fr : {♦} ⊑ φ).
+
+  (* Elimination on TPair *)
+  Example inst_fst1 : has_type Γ φ Σ (ttapp (ttapp fst)) ({(TPair A a a B b b b) | a ⊔ b ⊔ {♦}} ==> { A | a }) (a ⊔ b).
+    unfold TPair.
+    change_qual (openq a b (a ⊔ #!1)).
+    change_type (open_ty TUnit ∅ B b (
+      {∀<:{⊤ | a ⊔ #!1 ⊔ {♦}}.{
+        {{A | a} ==> {{#5 | #!5} ==> {# 5 | #! 5} | #! 1} | ∅} ==> {# 3 | #! 3} | #! 1 ⊔ a ⊔ #!3}
+          | a ⊔ #!1 ⊔ {♦}} ==> {A | a})).
+    apply t_tapp_fresh with (d1':=b ⊔ {♦}) (df':=a ⊔ {♦}); try solve [ccrush].
+    (* change bound *)
+    apply t_sub with (d1:=a) (T1:=(∀<:{⊤ | a ⊔ {♦}}.{
+      {∀<:{⊤ | a ⊔ #! 1 ⊔ {♦}}.{
+          {{A | a} ==> {{# 5 | #! 5} ==> {# 5 | #! 5} | #! 1} | ∅} ==> {# 3 | #! 3} | #! 1 ⊔ a ⊔ #! 3}
+      | a ⊔ #! 1 ⊔ {♦}} ==> {A | a}
+      | a ⊔ #! 1})); auto.
+    * change_qual (openq ∅ a #!1).
+      change_type (open_ty TUnit ∅ A a (∀<:{⊤ | #!1 ⊔ {♦}}.{
+        {∀<:{⊤ | #!3 ⊔ #! 1 ⊔ {♦}}.{
+            {{#5 | #!5} ==> {{# 5 | #! 5} ==> {# 5 | #! 5} | #! 1} | ∅} ==> {# 3 | #! 3} | #! 1 ⊔ #!5 ⊔ #! 3}
+                      | #!3 ⊔ #! 1 ⊔ {♦}} ==> {#5 | #!5} | #!3 ⊔ #! 1})).
+      apply t_tapp_fresh with (d1':=a ⊔ {♦}) (df':=∅); try solve [ccrush].
+      dom_equals ({♦}).
+      (* change bound *)
+      replace (#! 1 ⊔ {♦}) with (#♦1) at 1; try solve [ccrush].
+      replace (#! 3 ⊔ #! 1 ⊔ {♦}) with (#!1 ⊔ #!3 ⊔ {♦}) at 1; try solve [ccrush].
+      replace (#! 3 ⊔ #! 1) with (#!1 ⊔ #!3) at 1; try solve [ccrush].
+      eapply t_sub. eapply t_fst1. auto. unfold TPair. auto.
+      apply s_all. 1-4: ccrush. apply stp_refl; ccrush. apply qs_sq; ccrush. auto. auto. qual_destruct. ccrush.
+      intros. rewrite nf_a in H. discriminate. eauto.
+      inversion cl_a. inversion cl_b. subst. apply bound_0_empty in H0, H7. simpl in nf_a, nf_b. subst. ccrush.
+    * apply s_all. inversion cl_a. inversion cl_b. subst. apply bound_0_empty in H0, H7. simpl in nf_a, nf_b. subst. ccrush.
+      constructor. ccrush. constructor; ccrush. bound_simpl. lia. ccrush. constructor; ccrush.
+      constructor; ccrush. bound_simpl. lia. constructor; ccrush. constructor; ccrush. bound_simpl. lia.
+      constructor; ccrush. bound_simpl. lia.
+      inversion cl_a. inversion cl_b. subst. apply bound_0_empty in H0, H7. simpl in nf_a, nf_b. subst. ccrush.
+      constructor. ccrush. constructor; ccrush. eapply Nat.le_trans. eapply inter_bound_min. lia. bound_simpl. lia.
+      eapply Nat.le_trans. eapply inter_bound_min. lia. constructor; ccrush. bound_simpl. lia. ccrush.
+      constructor; ccrush. constructor; ccrush. bound_simpl. lia. constructor; ccrush. constructor; ccrush.
+      bound_simpl. lia. constructor; ccrush. bound_simpl. lia. ccrush. ccrush.
+      apply stp_refl. qual_destruct. inversion cl_a. inversion cl_b. subst. apply bound_0_empty in H17, H7. simpl in nf_a, nf_b. subst. ccrush.
+      constructor. ccrush. constructor; ccrush. bound_simpl. lia. bound_simpl. lia. ccrush.
+      constructor; ccrush. constructor; ccrush. 1,2 : bound_simpl; lia. constructor; ccrush. 1,2: bound_simpl; lia. ccrush.
+      apply qs_sq; ccrush.
+    * eauto.
+    * qual_destruct. inversion cl_a. inversion cl_b. subst. apply bound_0_empty in H7, H17. simpl in nf_a, nf_b. subst. ccrush.
+    * intros. rewrite nf_b in H. discriminate.
+    * opening. eauto.
+    * eauto.
+    * qual_destruct. inversion cl_a. inversion cl_b. subst. apply bound_0_empty in H7, H17. simpl in nf_a, nf_b. subst. ccrush.
+  Qed.
+
+  (* Elimination on TPair *)
+  Example inst_snd1 : has_type Γ φ Σ (ttapp (ttapp snd)) ({(TPair A a a B b b b) | a ⊔ b ⊔ {♦}} ==> { B | b }) (a ⊔ b).
+    unfold TPair.
+    change_qual (openq a b (a ⊔ #!1)).
+    change_type (open_ty TUnit ∅ B b (
+      {∀<:{⊤ | a ⊔ #!1 ⊔ {♦}}.{
+        {{A | a} ==> {{#5 | #!5} ==> {# 5 | #! 5} | #! 1} | ∅} ==> {# 3 | #! 3} | #! 1 ⊔ a ⊔ #!3}
+          | a ⊔ #!1 ⊔ {♦}} ==> {#3 | #!3})).
+    apply t_tapp_fresh with (d1':=b ⊔ {♦}) (df':=a ⊔ {♦}); try solve [ccrush].
+    (* change bound *)
+    apply t_sub with (d1:=a) (T1:=(∀<:{⊤ | a ⊔ {♦}}.{
+      {∀<:{⊤ | a ⊔ #! 1 ⊔ {♦}}.{
+          {{A | a} ==> {{# 5 | #! 5} ==> {# 5 | #! 5} | #! 1} | ∅} ==> {# 3 | #! 3} | #! 1 ⊔ a ⊔ #! 3}
+      | a ⊔ #! 1 ⊔ {♦}} ==> {#3 | #!3}
+      | a ⊔ #! 1})); auto.
+    * change_qual (openq ∅ a #!1).
+      change_type (open_ty TUnit ∅ A a (∀<:{⊤ | #!1 ⊔ {♦}}.{
+        {∀<:{⊤ | #!3 ⊔ #! 1 ⊔ {♦}}.{
+            {{#5 | #!5} ==> {{# 5 | #! 5} ==> {# 5 | #! 5} | #! 1} | ∅} ==> {# 3 | #! 3} | #! 1 ⊔ #!5 ⊔ #! 3}
+                      | #!3 ⊔ #! 1 ⊔ {♦}} ==> {#3 | #!3} | #!3 ⊔ #! 1})).
+      apply t_tapp_fresh with (d1':=a ⊔ {♦}) (df':=∅); try solve [ccrush].
+      dom_equals ({♦}).
+      (* change bound *)
+      replace (#! 1 ⊔ {♦}) with (#♦1) at 1; try solve [ccrush].
+      replace (#! 3 ⊔ #! 1 ⊔ {♦}) with (#!1 ⊔ #!3 ⊔ {♦}) at 1; try solve [ccrush].
+      replace (#! 3 ⊔ #! 1) with (#!1 ⊔ #!3) at 1; try solve [ccrush].
+      eapply t_sub. eapply t_snd1. auto. unfold TPair.
+      apply s_all. 1-4: ccrush. apply stp_refl; ccrush. apply qs_sq; ccrush. auto. auto. qual_destruct. ccrush.
+      intros. rewrite nf_a in H. discriminate. eauto.
+      inversion cl_a. inversion cl_b. subst. apply bound_0_empty in H0, H7. simpl in nf_a, nf_b. subst. ccrush.
+    * apply s_all. inversion cl_a. inversion cl_b. subst. apply bound_0_empty in H0, H7. simpl in nf_a, nf_b. subst. ccrush.
+      constructor. ccrush. constructor; ccrush. bound_simpl. lia. ccrush. constructor; ccrush.
+      constructor; ccrush. bound_simpl. lia. constructor; ccrush. constructor; ccrush. bound_simpl. lia.
+      constructor; ccrush. bound_simpl. lia.
+      inversion cl_a. inversion cl_b. subst. apply bound_0_empty in H0, H7. simpl in nf_a, nf_b. subst. ccrush.
+      constructor. ccrush. constructor; ccrush. eapply Nat.le_trans. eapply inter_bound_min. lia. bound_simpl. lia.
+      eapply Nat.le_trans. eapply inter_bound_min. lia. constructor; ccrush. bound_simpl. lia. ccrush.
+      constructor; ccrush. constructor; ccrush. bound_simpl. lia. constructor; ccrush. constructor; ccrush.
+      bound_simpl. lia. constructor; ccrush. bound_simpl. lia. ccrush. ccrush.
+      apply stp_refl. qual_destruct. inversion cl_a. inversion cl_b. subst. apply bound_0_empty in H17, H7. simpl in nf_a, nf_b. subst. ccrush.
+      constructor. ccrush. constructor; ccrush. bound_simpl. lia. bound_simpl. lia. ccrush.
+      constructor; ccrush. constructor; ccrush. 1,2 : bound_simpl; lia. constructor; ccrush. 1,2: bound_simpl; lia. ccrush.
+      apply qs_sq; ccrush.
+    * eauto.
+    * qual_destruct. inversion cl_a. inversion cl_b. subst. apply bound_0_empty in H7, H17. simpl in nf_a, nf_b. subst. ccrush.
+    * intros. rewrite nf_b in H. discriminate.
+    * opening. eauto.
+    * eauto.
+    * qual_destruct. inversion cl_a. inversion cl_b. subst. apply bound_0_empty in H7, H17. simpl in nf_a, nf_b. subst. ccrush.
+  Qed.
+
+  Example inst_pair1 : has_type Γ φ Σ (ttapp (ttapp pair_mk)) ({A | a} ==> {{B | b} ==> {TPair A #!3 #!5 B #!1 #!3 #!5 | #!1 ⊔ #!3 } | #!1 }) (a ⊔ b).
+    unfold TPair.
+    change_qual (openq a b (a ⊔ #!1)).
+    change_type (open_ty TUnit ∅ B b
+    ({A | a}
+          ==> {{#3 | #!3}
+                  ==> {∀<:{⊤ | #! 3 ⊔ #! 1 ⊔ {♦}}.{
+                          {{A | #! 5} ==> {{#9 | #! 5} ==> {# 5 | #! 5} | #! 1} | ∅} ==> {# 3 | #! 3}
+                          | #! 1 ⊔ #! 5 ⊔ #! 3}
+                      | #! 1 ⊔ #! 3}
+              | #! 1})).
+    apply t_tapp_fresh with (d1':=b ⊔ {♦}) (df':=a ⊔ {♦}); try solve [ccrush].
+    (* change the bound *)
+    eapply t_sub with (T1:=(∀<:{⊤ | a ⊔ {♦}}.{
+      {A | a}
+         ==> {{# 3 | #! 3}
+                 ==> {∀<:{⊤ | #! 3 ⊔ #! 1 ⊔ {♦}}.{
+                         {{A | #! 5} ==> {{# 9 | #! 5} ==> {# 5 | #! 5} | #! 1} | ∅}
+                            ==> {# 3 | #! 3}
+                         | #! 1 ⊔ #! 5 ⊔ #! 3}
+                     | #! 1 ⊔ #! 3}
+             | #! 1}
+      | a ⊔ #! 1}) ) (d1:=a); auto.
+    * change_qual (openq ∅ a #!1).
+      change_type (open_ty TUnit (∅) A a (∀<:{⊤ | #!1 ⊔ {♦}}.{
+        {#3 | #!3}
+           ==> {{# 3 | #! 3}
+                   ==> {∀<:{⊤ | #! 3 ⊔ #! 1 ⊔ {♦}}.{
+                           {{#9 | #! 5} ==> {{# 9 | #! 5} ==> {# 5 | #! 5} | #! 1} | ∅}
+                              ==> {# 3 | #! 3}
+                           | #! 1 ⊔ #! 5 ⊔ #! 3}
+                       | #! 1 ⊔ #! 3}
+               | #! 1}
+        | #!3 ⊔ #! 1})).
+      eapply t_tapp_fresh with (d1':=a ⊔ {♦}) (df':=∅); try solve [ccrush]. dom_equals ({♦}).
+      (* change the bound *)
+      eapply t_sub with (T1:=(∀<:{⊤ | {♦}}.{
+        ∀<:{⊤ | #♦1}.{
+           {# 3 | #! 3}
+              ==> {{# 3 | #! 3}
+                      ==> {∀<:{⊤ | #! 3 ⊔ #! 1 ⊔ {♦}}.{
+                              {{# 9 | #! 5} ==> {{# 9 | #! 5} ==> {# 5 | #! 5} | #! 1} | ∅}
+                                 ==> {# 3 | #! 3}
+                              | #! 1 ⊔ #! 5 ⊔ #! 3}
+                          | #! 3 ⊔ #! 1}
+                  | #! 1}
+           | #! 1 ⊔ #! 3}
+        | #!1})) (d1:=∅); auto.
+      apply t_pair1. auto.
+      apply s_all. ccrush. ccrush. ccrush. ccrush. cleanup; try lia. apply s_all. ccrush. ccrush. apply qs_sq; ccrush.
+      apply stp_refl; ccrush. apply qs_sq; ccrush. replace (union (singleton 1) (singleton 3)) with (union (singleton 3) (singleton 1)).
+      apply stp_refl; ccrush. apply qs_sq; ccrush. fnsetdec.
+      qual_destruct. ccrush. intros. rewrite H in nf_a. discriminate. eauto.
+      opening. ccrush. qual_destruct. cleanup. f_equal. qdec. qdec.
+    * apply s_all. 1-4: ccrush. apply stp_refl; ccrush. apply qs_sq; ccrush.
+    * eauto.
+    * intros. rewrite H in nf_b. discriminate.
+    * opening. eauto.
+    * eauto.
+    * cleanup. qual_destruct. repeat f_equal; fnsetdec. all : lia.
+  Qed.
+
+  Section IntroElimExample.
+
+    Context (ta tb : tm)
+            (ht_ta : has_type Γ φ Σ ta A a)
+            (ht_tb : has_type Γ φ Σ tb B b).
+
+    (* pair_mk[A,B](ta,tb) *)
+    Example pair_ab := (tapp (tapp (ttapp (ttapp pair_mk)) ta) tb).
+
+    Example pair_intro1 :
+      has_type Γ φ Σ pair_ab (TPair A a a B b b b) (a ⊔ b).
+      intros. unfold pair_ab. unfold TPair.
+      change_qual (openq a b (a ⊔ #!1)).
+      change_type (open_ty TUnit ∅ B b (∀<:{⊤ | a ⊔ #!1 ⊔ {♦}}.{
+        {{A | a} ==> {{B | #!5} ==> {# 5 | #! 5} | #! 1} | ∅} ==> {# 3 | #! 3} | #! 1 ⊔ a ⊔ #!3})).
+      apply t_app; try solve [ccrush].
+      change_qual (openq (a ⊔ b) a #!1). replace (a ⊔ #! 1) with (#!1 ⊔ a).
+      change_type (open_ty TUnit ∅ A a (
+        {B | b}
+          ==> {∀<:{⊤ | #!3 ⊔ #! 1 ⊔ {♦}}.{
+              {{A | #!5} ==> {{B | #! 5} ==> {# 5 | #! 5} | #! 1} | ∅} ==> {# 3 | #! 3}
+              | #! 1 ⊔ #!5 ⊔ #! 3}
+          | #!1 ⊔ #! 3})).
+      apply t_app; auto. apply inst_pair1. ccrush. ccrush. ccrush. qual_destruct.
+      inversion cl_b. inversion cl_a. subst. apply bound_0_empty in H7, H17. subst. opening. cleanup. simpl in nf_a. simpl in nf_b. subst.
+      auto. 1-6: lia. rewrite qlub_commute. auto. qual_destruct. inversion cl_a. subst. apply bound_0_empty in H7. subst. simpl in nf_a. subst.
+      ccrush. opening. eauto.
+      opening. cleanup. qual_destruct. cleanup. inversion cl_a. subst. apply bound_0_empty in H7. subst. cleanup.
+      simpl in nf_a. simpl in nf_b. subst. repeat f_equal. all: lia.
+    Qed.
+
+    (* fst[A,B](pair_ab) : A^a *)
+    Example pair1_elim1 : has_type Γ φ Σ (tapp (ttapp (ttapp fst)) pair_ab) A a.
+      change_qual (openq (a ⊔ b) (a ⊔ b) a).
+      change_type (open_ty TUnit (∅) (TPair A a a B b b b) (a ⊔ b) A).
+      apply t_app_fresh with (d1':=(a⊔ {♦})⊔(b⊔{♦})) (df':=(a⊔ {♦})⊔(b⊔{♦})) ; try solve [ccrush].
+      * dom_equals (a ⊔ b ⊔ {♦}). apply inst_fst1. qual_destruct. simpl.
+        simpl in nf_a, nf_b. subst. qdec.
+      * apply pair_intro1.
+      * intros. qual_destruct. simpl in *. rewrite nf_a in H. rewrite nf_b in H. simpl in H. discriminate.
+    Qed.
+
+    (* snd[A,B](pair_ab) : A^b *)
+    Example pair1_elim2 : has_type Γ φ Σ (tapp (ttapp (ttapp snd)) pair_ab) B b.
+      change_qual (openq (a ⊔ b) (a ⊔ b) b).
+      change_type (open_ty TUnit (∅) (TPair A a a B b b b) (a ⊔ b) B).
+      apply t_app_fresh with (d1':=(a⊔ {♦})⊔(b⊔{♦})) (df':=(a⊔ {♦})⊔(b⊔{♦})) ; try solve [ccrush].
+      * dom_equals (a ⊔ b ⊔ {♦}). apply inst_snd1. qual_destruct. simpl.
+        simpl in nf_a, nf_b. subst. qdec.
+      * apply pair_intro1.
+      * intros. qual_destruct. simpl in *. rewrite nf_a in H. rewrite nf_b in H. simpl in H. discriminate.
+    Qed.
+
+  End IntroElimExample.
+
+End PairTransparentUse.
+
+Section PairTransparentConcreteUse.
+  (* A more concrete usage example, shown in Section 2.4 of the paper *)
+
+  Variables (φ : qual) (Σ : senv).
+
+  Definition TRefU := TRef ∅ TUnit.
+
+
+  Definition Γ : tenv := [ bind_tm (false, TRefU, {♦}) ; bind_tm (false, TRefU, {♦}) ].
+
+  Example u := $0.
+  Example v := $1.
+  Example qu := $! 0.
+  Example qv := $! 1.
+
+  Context (phiwf : closed_qual 0 (‖Γ‖) (‖Σ‖) φ)
+          (qu_obs : qu ⊑ φ)
+          (qv_obs : qv ⊑ φ)
+          (phi_fr : {♦} ⊑ φ)
+          (sat : senv_saturated Σ ∅).
+
+   (* Section 2.4:
+      (tlet (tref tunit) (* u*)
+        (tlet (tref tunit) (* v *)
+            (tlet (pair u v) (* p *)
+              (fst p) ; (snd p)
+   *)
+  Example pair_uv := (tapp (tapp (ttapp (ttapp pair_mk)) u) v).
+
+  (* pair_uv : Pair[Ref[Unit]^u, Ref[Unit]^v]^{u,v}*)
+  Example pair_uv_ty : has_type Γ φ Σ pair_uv (TPair TRefU qu qu TRefU qv qv qv) (qu ⊔ qv).
+  Proof.
+    apply pair_intro1; ccrush.
+    econstructor. auto. auto. econstructor. auto. auto.
+    eapply t_var. simpl. auto. auto. auto. unfold TRefU.
+    econstructor. auto. auto. auto.
+    eapply t_var. simpl. auto. auto. auto. unfold TRefU.
+    econstructor. auto. auto. auto.
+  Qed.
+
+  (*
+     In context p : Pair[Ref[Unit]^u, Ref[Unit]^v]^p
+     we have that fst(p): Ref[Unit]^u
+  *)
+  Example proj1_fst :
+  has_type
+    (bind_tm (false, TPair TRefU qu qu TRefU qv qv qv, qu ⊔ qv)
+     :: bind_tm (true, {TPair TRefU qu qu TRefU qv qv qv | qu ⊔ qv} ==> {TRef ∅ TUnit | $! 0},
+           qu ⊔ qv) :: Γ)
+    (qset true (union (union (singleton 0) (singleton 1)) (union (singleton 2) (singleton 3))) {}N {}N)
+    Σ
+    (tapp (ttapp (ttapp fst)) $ 3)
+    (TRef ∅ TUnit) $! 0.
+  Proof.
+    change_qual (openq (qu ⊔ qv) (qu ⊔ qv) qu).
+    change_type (open_ty TUnit ∅ (TPair TRefU qu qu TRefU qv qv qv) (qu ⊔ qv) (TRef ∅ TUnit)).
+    apply t_app_fresh with (d1':=(qu ⊔ {♦})⊔(qv ⊔{♦})) (df':=(qu ⊔ {♦})⊔(qv ⊔{♦})) ; try solve [ccrush].
+    - dom_equals (qu ⊔ qv ⊔ {♦}). apply inst_fst1; ccrush. unfold qu. ccrush. unfold qv. ccrush.
+      unfold TRefU. ccrush.
+    - eapply t_sub. eapply t_var; ccrush. unfold TPair. unfold TRefU. unfold qu. unfold qv. ccrush.
+      apply stp_refl; try solve [unfold TPair; unfold TRefU; unfold qu; unfold qv; ccrush].
+      eapply qs_qvar; try solve [unfold TPair; unfold TRefU; unfold qu; unfold qv; ccrush].
+      ccrush. ccrush.
+    - constructor; eauto. unfold tenv_saturated. intros.
+      repeat rewrite qmem_lub_or_commute in H. destruct H.
+      simpl in H. destruct H. apply NatSetFacts.singleton_iff in H; subst.
+      try solve [eapply sat_tvar; ccrush]; try solve [eapply sat_var; ccrush]. ccrush.
+      simpl in H. destruct H. apply NatSetFacts.singleton_iff in H; subst.
+      try solve [eapply sat_tvar; ccrush]; try solve [eapply sat_var; ccrush]. ccrush.
+      unfold senv_saturated. intros.
+      repeat rewrite qmem_lub_or_commute in H. destruct H.
+      simpl in H. destruct H; ccrush. simpl in H. destruct H; ccrush.
+    - constructor; eauto. unfold tenv_saturated. intros.
+      repeat rewrite qmem_lub_or_commute in H. destruct H.
+      simpl in H. destruct H. apply NatSetFacts.singleton_iff in H; subst.
+      try solve [eapply sat_tvar; ccrush]; try solve [eapply sat_var; ccrush]. ccrush.
+      simpl in H. destruct H. apply NatSetFacts.singleton_iff in H; subst.
+      try solve [eapply sat_tvar; ccrush]; try solve [eapply sat_var; ccrush]. ccrush.
+      unfold senv_saturated. intros.
+      repeat rewrite qmem_lub_or_commute in H. destruct H.
+      simpl in H. destruct H; ccrush. simpl in H. destruct H; ccrush.
+  Qed.
+
+  (*
+  u: Ref^♦, v: Ref^♦ |- let p = pair u v in (fst p) : Ref^u
+  *)
+  Example proj1 : has_type Γ φ Σ (tlet pair_uv (tapp (ttapp (ttapp fst)) #1)) (TRef ∅ TUnit) qu.
+  Proof.
+    unfold pair_uv. unfold u. unfold v. unfold tlet.
+    change_qual (openq (qu ⊔ qv) (qu ⊔ qv) qu).
+    change_type (open_ty TUnit ∅ (TPair TRefU qu qu TRefU qv qv qv) (qu ⊔ qv) (TRef ∅ TUnit)).
+    unfold qu. unfold qv.
+    eapply t_app.
+    - eapply t_abs; ccrush. econstructor; ccrush.
+      econstructor; ccrush. econstructor; ccrush. econstructor; ccrush.
+      econstructor; ccrush. econstructor; ccrush. econstructor; ccrush.
+      fold fst. fold qu. fold qv.
+      replace (qset false (union (singleton 0) (singleton 1)) {}N {}N) with (qu ⊔ qv).
+      eapply proj1_fst. simpl. ccrush.
+    - apply pair_uv_ty.
+    - ccrush.
+    - ccrush.
+    - ccrush.
+    - ccrush.
+  Qed.
+
+End PairTransparentConcreteUse.
+
+Section PairOpaque.
+  (*
+      We now cover _opaque_ pairs with components reaching out-of-scope variables. It is recommended to review
+      examples_cell_opaque.v first for the basic idea.
+
+      Opaque pairs have the following shape:
+
+      OPair[A,B] := p∀C^c<:⊤^∅. f(g(x:A^♦ -> (y:B^x,♦ -> C^x,y)^x)^∅ -> C^f)^p
+
+      With the addition of a second datum, the extractor function is now a dependent function of the form
+
+      g(x:A^♦ -> (y:B^x,♦ -> C^x,y)
+
+      which accepts the two (contextually fresh) components. Note that we permit potential overlap at
+      y with x. The result is C and may reach both x and y. Essentially, this encoding, due to ignoring
+      the qualifier binder c, behaves like the "imprecise" pairs in Section 2.3 of the paper.
+      Is this an issue? Not at all in the case of out-of-scope data, because all we know is that the
+      data will reach the name of the pair anyway.
+      Using the same "self-reference chain" trick introduced in examples_cell_opaque.v, we demonstrate
+      this in the following:
+
+      pair: (p∀C^c<:⊤^∅. f(g(x:A^♦ -> (y:B^x,♦ -> C^x,y)^x)^∅ -> C^f)^p)^pair ⊣ pair : OPair[A,B]^♦
+
+      pair[A^∅]: f(g(x:A^♦ -> (y:B^x,♦ -> A^x,y)^x)^∅ -> A^f)^pair
+      pair[B^∅]: f(g(x:A^♦ -> (y:B^x,♦ -> B^x,y)^x)^∅ -> B^f)^pair
+
+      pair[A^∅](x => y => x) : A^pair
+      pair[B^∅](x => y => x) : B^pair
+  *)
+
+
+  (*
+    OPair[A,B] := p∀C^c<:⊤^∅. f(g(x:A^♦ -> (y:B^x,♦ -> C^x,y)^x)^∅ -> C^f)^p
+    Note: the number attached to each parameter indicates by how much it must be incremented if it is a deBruijn index.
+  *)
+  Example TOPair A2 B4 := (∀<:{ ∅ }.{ { { A2 | {♦} } ==> { { B4 | #♦1 } ==> {  #5  | #!3 ⊔ #!1  } | #!1 } | ∅ } ==> { #3 | #!0 } | #!0 }).
+
+  (* Opaque pair introduction typing
+    ([A^a<:⊤^♦] => ([B^b<:⊤♦a] => (g(x: A^a) => (h(y: B^b) => TOPair[A,B]^x,y,a,b)^x,a,b )^a,b )^a )^∅ *)
+  Example t_pair_mk_ :
+    has_type [] ∅ [] pair_mk (∀.{ ∀<:{ #♦1 }.{ {#3 | #!3 } ==> { {#3 | #!3} ==> {TOPair #9 #9 | #!1 ⊔ #!3 ⊔ #!5 ⊔ #!7 } | #!1 ⊔ #!3 ⊔ #!5 } | #!1 ⊔ #!3 } | #!1  }) ∅.
+  Proof.
+    unfold pair_mk.
+    apply t_tabs; ccrush. unfold TOPair. ccrush. (* 0/1*)
+    apply t_tabs; ccrush. (* 2/3 *)
+    apply t_abs; ccrush. (* 4/5 *)
+    apply t_abs; ccrush. (* 6/7 *)
+    apply t_tabs; ccrush. (* 8/9 *)
+    (* p abstraction *)
+    (* x,y,a,b <: p *)
+    eapply t_sub with (d1:=$!1 ⊔ $!3 ⊔ $!5 ⊔ $!7).
+    2: {
+        eapply stp_refl; try solve [ccrush].
+        apply qs_trans with (d2:=($! 1 ⊔ $! 3 ⊔ $! 5 ⊔ $! 7) ⊔ $!8).
+        apply qs_sq; ccrush. eapply qs_self_all; ccrush.
+        f_equal. f_equal. f_equal. qdec.
+    } 2,3 : ccrush.
+    apply t_abs; ccrush.  (* 10/11 *)
+    (* f abstraction: *)
+    (* a,y <: x,y,a,b <: f*)
+    eapply t_sub with (d1:=$!1 ⊔ $!7).
+    2 : {
+        eapply stp_refl; try solve [ccrush].
+        apply qs_trans with (d2:=($! 1 ⊔ $! 3 ⊔ $! 5 ⊔ $! 7) ⊔ $!10).
+        apply qs_sq; ccrush. eapply qs_self; ccrush.
+    } 2,3 : ccrush.
+    change_qual (openq $!1 $!7 ($!1 ⊔ #!1)).
+    change_type (open_ty TUnit (∅) ($3) $!7 $9).
+    apply t_app_fresh with (d1':=$!7⊔$!3⊔$♦1) (df':=$♦1); try solve [ccrush].
+    * dom_equals ($♦1).
+      change_qual (openq $!11 $!1 #!1).
+      change_type (open_ty TUnit (∅) $1 $!1 ({$ 3 | #♦1} ==> {$ 9 | #! 3 ⊔ #! 1})).
+      eapply t_app_fresh with (d1':=$♦1) (df':=$!11); try solve [ccrush].
+      + dom_equals ({♦}). eapply t_var; ccrush.
+      + eapply t_sub. eapply t_var; ccrush.
+        apply stp_refl; ccrush. eapply qs_qvar; ccrush. all : ccrush.
+    * eapply t_var; ccrush.
+    * (* show transitive reachability closure of this qualifier, could be further automated *)
+      constructor; eauto. unfold tenv_saturated. intros.
+      repeat rewrite qmem_lub_or_commute in H. destruct H as [  Hmem | [ Hmem  | Hmem] ];
+      simpl in Hmem; apply NatSetFacts.singleton_iff in Hmem; subst;
+      try solve [eapply sat_tvar; ccrush]; try solve [eapply sat_var; ccrush].
+  Qed.
+
+  (* generalize to all contexts *)
+  Example t_pair_mk : forall {Γ φ Σ}, closed_qual 0 (‖Γ‖) (‖Σ‖) φ ->
+    has_type Γ φ Σ pair_mk (∀.{ ∀<:{ #♦1 }.{ {#3 | #!3 } ==> { {#3 | #!3} ==> {TOPair #9 #9 | #!1 ⊔ #!3 ⊔ #!5 ⊔ #!7 } | #!1 ⊔ #!3 ⊔ #!5 } | #!1 ⊔ #!3 } | #!1  }) ∅.
+  Proof.
+    intros. eapply weaken'. eapply weaken_store. apply t_pair_mk_. all : auto.
+  Qed.
+
+  (* The extractors (Church booleans) are compatible with the extractor signature of OPair: *)
+  (* λx.λy.x : (x:A^♦ => (y:B^♦,x => A^xy)^x)^∅ *)
+  Example elim1 : forall Γ φ Σ A B,
+    closed_qual 0 (‖ Γ ‖) (‖ Σ ‖) φ ->
+    closed_ty 0 (‖ Γ ‖) (‖ Σ ‖) A ->
+    closed_ty 0 (‖ Γ ‖) (‖ Σ ‖) B ->
+    has_type Γ φ Σ (tabs (tabs #3)) ({ A | {♦} } ==> { {B | #♦1 } ==> {A | #!3 ⊔ #!1 } | #!1 }) ∅.
+  Proof.
+    intros.
+    apply t_abs; ccrush.
+    apply t_abs; ccrush.
+    eapply t_sub. eapply t_var; ccrush.
+    apply stp_refl; ccrush. apply qs_sq; ccrush. all : ccrush.
+  Qed.
+
+  (* λx.λy.y : (x:A^♦ => (y:B^♦,x => B^xy)^x)^∅ *)
+  Example elim2 : forall Γ φ Σ A B,
+    closed_qual 0 (‖ Γ ‖) (‖ Σ ‖) φ ->
+    closed_ty 0 (‖ Γ ‖) (‖ Σ ‖) A ->
+    closed_ty 0 (‖ Γ ‖) (‖ Σ ‖) B ->
+    has_type Γ φ Σ (tabs (tabs #1)) ({ A | {♦} } ==> { {B | #♦1 } ==> {B | #!3 ⊔ #!1 } | #!1 }) ∅.
+  Proof.
+    intros.
+    apply t_abs; ccrush.
+    apply t_abs; ccrush.
+    eapply t_sub. eapply t_var; ccrush.
+    apply stp_refl; ccrush. apply qs_sq; ccrush. all : ccrush.
+  Qed.
+
+  (* OPair elimination typing
+     fst: ([A^a <: ⊤^♦] => ([B^b <: ⊤^♦a] => (OPair[A,B]^{a,b} => A^a,b)^a,b)^a)^∅ *)
+  Example t_fst_ :
+    has_type [] ∅ [] fst (∀.{ ∀<:{ #♦1 }.{ {TOPair #5 #5 | #!1 ⊔ #!3 } ==> { #5 | #!3 ⊔ #!5 } | #!1 ⊔ #!3 } | #!1 }) ∅.
+  Proof.
+    unfold fst.
+    apply t_tabs; ccrush. unfold TOPair. ccrush.
+    apply t_tabs; ccrush.
+    apply t_abs; ccrush.
+    change_qual (openq (qset false (union (singleton 1) (singleton 3)) {}N {}N) (∅) #!0).
+    change_type (open_ty TUnit (∅) ({$ 1 | {♦}} ==> {{$ 3 | #♦1 } ==> {$1 | #!3 ⊔ #!1 } | #!1}) (∅) $1).
+    apply t_app; try solve [ccrush].
+    * change_qual (openq (qset false (union (singleton 1) (singleton 3)) {}N {}N) ∅ #!0).
+      change_type (open_ty TUnit ∅ $1 ∅ ({{$ 1 | {♦}} ==> {{$ 3 | #♦1 } ==> {# 5 | #!3 ⊔ #! 1 } | #!1 } | ∅ } ==> {# 3 | #! 0})).
+      apply t_tapp; ccrush.
+      eapply t_sub.
+      eapply t_var; ccrush.
+      apply s_all. ccrush. ccrush.
+      eapply qs_qvar; ccrush.
+      eapply s_tvar_trans; ccrush. cleanup. apply stp_refl; ccrush. eapply qs_sq; ccrush.
+      all : ccrush.
+    * apply elim1; ccrush.
+  Qed.
+
+  (* generalize to all contexts *)
+  Example t_fst : forall {Γ φ Σ}, closed_qual 0 (‖Γ‖) (‖Σ‖) φ ->
+    has_type Γ φ Σ fst (∀.{ ∀<:{ #♦1 }.{ {TOPair #5 #5 | #!1 ⊔ #!3 } ==> { #5 | #!3 ⊔ #!5 } | #!1 ⊔ #!3 } | #!1 }) ∅.
+  Proof.
+    intros. eapply weaken'. eapply weaken_store. apply t_fst_. all : auto.
+  Qed.
+
+   (* OPair elimination typing
+      snd: ([A^a <: ⊤^♦] => ([B^b <: ⊤^♦a] => (OPair[A,B]^{a,b} => B^a,b)^a,b)^a)^∅ *)
+  Example t_snd_ :
+    has_type [] ∅ [] snd (∀.{ ∀<:{ #♦1 }.{ {TOPair #5 #5 | #!1 ⊔ #!3 } ==> { #3 | #!3 ⊔ #!5 } | #!1 ⊔ #!3 } | #!1 }) ∅.
+  Proof.
+    unfold snd.
+    apply t_tabs; ccrush. unfold TOPair. ccrush.
+    apply t_tabs; ccrush.
+    apply t_abs; ccrush.
+    change_qual (openq (qset false (union (singleton 1) (singleton 3)) {}N {}N) (∅) #!0).
+    change_type (open_ty TUnit (∅) ({$ 1 | {♦}} ==> {{$ 3 | #♦1 } ==> {$3 | #!3 ⊔ #!1 } | #!1}) (∅) $3).
+    apply t_app; try solve [ccrush].
+    * change_qual (openq (qset false (union (singleton 1) (singleton 3)) {}N {}N) ∅ #!0).
+      change_type (open_ty TUnit ∅ $3 ∅ ({{$ 1 | {♦}} ==> {{$ 3 | #♦1 } ==> {# 5 | #!3 ⊔ #! 1 } | #!1 } | ∅ } ==> {# 3 | #! 0})).
+      apply t_tapp; ccrush.
+      eapply t_sub.
+      eapply t_var; ccrush.
+      apply s_all. ccrush. ccrush.
+      eapply qs_qvar; ccrush.
+      eapply s_tvar_trans; ccrush. cleanup. apply stp_refl; ccrush. eapply qs_sq; ccrush.
+      all : ccrush.
+    * apply elim2; ccrush.
+  Qed.
+
+  (* generalize to all contexts *)
+  Example t_snd : forall {Γ φ Σ}, closed_qual 0 (‖Γ‖) (‖Σ‖) φ ->
+    has_type Γ φ Σ snd (∀.{ ∀<:{ #♦1 }.{ {TOPair #5 #5 | #!1 ⊔ #!3 } ==> { #3 | #!3 ⊔ #!5 } | #!1 ⊔ #!3 } | #!1 }) ∅.
+  Proof.
+    intros. eapply weaken'. eapply weaken_store. apply t_snd_. all : auto.
+  Qed.
+
+End PairOpaque.
+
+Section OpaquePairUse.
+
+  (* a concrete use of opaque pairs *)
+
+  Context (Σ := [(TUnit, ∅); ({ TUnit | ∅} ==> {TUnit | ∅}, ∅)])
+          (φ := ({♦} ⊔ &!0 ⊔ &!1)).
+
+  (* pair_mk(&0,&1)    *)
+  Example pair_of_refs := (tapp (tapp (ttapp (ttapp pair_mk)) &0) &1).
+  Example fst_pair_of_refs := (tapp (ttapp (ttapp fst)) pair_of_refs).
+  Example snd_pair_of_refs := (tapp (ttapp (ttapp snd)) pair_of_refs).
+
+  (* some auxiliary lemmas stating that the singleton locations are transitively reachability closed. *)
+  Lemma sat_loc_1: saturated [] Σ &!1.
+  Proof.
+    unfold Σ. constructor; eauto.
+    unfold senv_saturated. intros. simpl in H; apply NatSetFacts.singleton_iff in H; subst.
+    apply sat_loc with (U:=TUnit) (q':=∅); ccrush.
+    Unshelve. auto.
+  Qed.
+
+  Lemma sat_loc_0: saturated [] Σ &!0.
+  Proof.
+    unfold Σ. constructor; eauto.
+    unfold tenv_saturated. intros. simpl in H. fnsetdec.
+    unfold senv_saturated. intros. simpl in H; apply NatSetFacts.singleton_iff in H; subst.
+    eapply sat_loc; ccrush.
+  Qed.
+
+  (* Instantiation typing of fst for this example
+     fst : OPair[Ref[Unit => Unit],Ref[Unit]]^{&0,&1} => Ref[Unit => Unit]^{&0,&1}
+  *)
+  Example t_fst_inst: has_type [] φ Σ (ttapp (ttapp fst)) ({TOPair (TRef ∅ ({TUnit | ∅} ==> {TUnit | ∅})) (TRef ∅ TUnit) | &!0 ⊔ &!1 } ==> { (TRef ∅ ({TUnit | ∅} ==> {TUnit | ∅})) | &!0 ⊔ &!1 }) (&!0 ⊔ &!1).
+  Proof.
+    change_qual (openq &!0 &!1 (&!0 ⊔ #!1)).
+    change_type (open_ty TUnit ∅ (TRef ∅ TUnit) &!1
+                  ({TOPair (TRef ∅ ({TUnit | ∅} ==> {TUnit | ∅})) #5 | #! 1 ⊔ &! 0} ==> {TRef ∅ ({TUnit | ∅} ==> {TUnit | ∅}) | &! 0 ⊔ #!3})).
+    2 : unfold TOPair; cleanup.
+    eapply t_tapp_fresh with (d1':=&!1) (df':=&!0) ; try solve [unfold TOPair; ccrush].
+    dom_equals ({♦}). apply (t_sub_bound ⊤ &♦0); try solve [ccrush].
+    change_qual (openq ∅ &!0 #!1).
+    change_type (open_ty TUnit ∅ (TRef ∅ ({TUnit | ∅} ==> {TUnit | ∅})) &!0
+                                 (∀<:{⊤ | #♦1}.{
+                                      {TOPair #5 # 5 | #! 1 ⊔ #!3}
+                                          ==> {#5 | #!5 ⊔ #! 3} | #!3 ⊔ #! 1})).
+    2: unfold TOPair; ccrush.
+    apply t_tapp_fresh with (d1':=&!0) (df':=∅); try solve [ccrush].
+    dom_equals ({♦}). apply (t_sub_bound ⊤ {♦}); try solve [ccrush].
+    replace (#! 5 ⊔ #! 3) with (#!3 ⊔ #!5); try solve [ccrush].
+    replace (#! 3 ⊔ #! 1) with (#!1 ⊔ #!3); try solve [ccrush].
+    apply t_fst; ccrush.
+    all : ccrush. all: eauto using sat_loc_1, sat_loc_0.
+  Qed.
+
+  (* Instantiation typing of snd for this example
+     snd : OPair[Ref[Unit => Unit],Ref[Unit]]^{&0,&1} => Ref[Unit]^{&0,&1}
+  *)
+  Example t_snd_inst: has_type [] φ Σ (ttapp (ttapp snd)) ({TOPair (TRef ∅ ({TUnit | ∅} ==> {TUnit | ∅})) (TRef ∅ TUnit) | &!0 ⊔ &!1 } ==> { (TRef ∅ TUnit) | &!0 ⊔ &!1 }) (&!0 ⊔ &!1).
+  Proof.
+    change_qual (openq &!0 &!1 (&!0 ⊔ #!1)).
+    change_type (open_ty TUnit ∅ (TRef ∅ TUnit) &!1
+                  ({TOPair (TRef ∅ ({TUnit | ∅} ==> {TUnit | ∅})) #5 | #! 1 ⊔ &! 0} ==> {#3 | &! 0 ⊔ #!3})).
+    2 : unfold TOPair; cleanup.
+    eapply t_tapp_fresh with (d1':=&!1) (df':=&!0) ; try solve [unfold TOPair; ccrush].
+    dom_equals ({♦}). apply (t_sub_bound ⊤ &♦0); try solve [ccrush].
+    change_qual (openq ∅ &!0 #!1).
+    change_type (open_ty TUnit ∅ (TRef ∅ ({TUnit | ∅} ==> {TUnit | ∅})) &!0
+                                 (∀<:{⊤ | #♦1}.{
+                                      {TOPair #5 # 5 | #! 1 ⊔ #!3}
+                                          ==> {#3 | #!5 ⊔ #! 3} | #!3 ⊔ #! 1})).
+    2: unfold TOPair; ccrush.
+    apply t_tapp_fresh with (d1':=&!0) (df':=∅); try solve [ccrush].
+    dom_equals ({♦}). apply (t_sub_bound ⊤ {♦}); try solve [ccrush].
+    replace (#! 5 ⊔ #! 3) with (#!3 ⊔ #!5); try solve [ccrush].
+    replace (#! 3 ⊔ #! 1) with (#!1 ⊔ #!3); try solve [ccrush].
+    apply t_snd; ccrush.
+    all : ccrush. all: eauto using sat_loc_1, sat_loc_0.
+  Qed.
+
+  (* Instantiation typing of the pair constructor for this example
+     pair_mk : Ref[Unit => Unit]^&0 => Ref[Unit]^&1 => OPair[Ref[Unit => Unit],Ref[Unit]]^{&0,&1}
+  *)
+  Example t_pair_mk_inst: has_type [] φ Σ (ttapp (ttapp pair_mk))
+                                ( {(TRef ∅ ({TUnit | ∅} ==> {TUnit | ∅})) | &!0 }
+                                   ==> { { (TRef ∅ TUnit) | &!1 }
+                                          ==> { TOPair (TRef ∅ ({TUnit | ∅} ==> {TUnit | ∅})) (TRef ∅ TUnit) | #!1 ⊔ #!3 ⊔ &!1 ⊔ &!0 } | #!1 ⊔ &!1 ⊔ &!0 }) (&!1 ⊔ &!0).
+  Proof.
+    change_qual (openq &!0 &!1 (#!1 ⊔ &!0)).
+    change_type (open_ty TUnit ∅ (TRef ∅ TUnit) &!1
+                    ({TRef ∅ ({TUnit | ∅} ==> {TUnit | ∅}) | &! 0}
+                         ==> {{#3 | #!3 }
+                                ==> {TOPair (TRef ∅ ({TUnit | ∅} ==> {TUnit | ∅})) #9 | #! 1 ⊔ #! 3 ⊔ #!5 ⊔ &! 0} | #! 1 ⊔ #!3 ⊔ &!0 })).
+    2 : { unfold TOPair; ccrush. f_equal. qdec. f_equal. qdec. }
+    eapply t_tapp_fresh with (d1':=&!1) (df':=&!0) ; try solve [unfold TOPair; ccrush].
+    dom_equals ({♦}). apply (t_sub_bound ⊤ &♦0); try solve [ccrush].
+    change_qual (openq ∅ &!0 #!1).
+    change_type (open_ty TUnit ∅ (TRef ∅ ({TUnit | ∅} ==> {TUnit | ∅})) &!0
+                                 (∀<:{⊤ | #♦1}.{
+                                      {#3 | #!3}
+                                          ==> {{# 3 | #! 3}
+                                               ==> {TOPair #9 # 9 | #! 1 ⊔ #! 3 ⊔ #!5 ⊔ #! 7} | #! 1 ⊔ #!3 ⊔ #!5 } | #!1 ⊔ #!3})).
+    2 : unfold TOPair; ccrush.
+    apply t_tapp_fresh with (d1':=&!0) (df':=∅); try solve [ccrush].
+    dom_equals ({♦}). apply (t_sub_bound ⊤ {♦}); try solve [ccrush].
+    apply t_pair_mk; ccrush.
+    all : ccrush. all: eauto using sat_loc_1, sat_loc_0.
+  Qed.
+
+  (* pair_of_refs : OPair[Ref[Unit => Unit],Ref[Unit]]^{&0,&1} *)
+  Example t_pair_of_refs: has_type [] φ Σ pair_of_refs (TOPair (TRef ∅ ({TUnit | ∅} ==> {TUnit | ∅})) (TRef ∅ TUnit)) (&!1 ⊔ &!0).
+  Proof.
+    unfold pair_of_refs.
+    change_qual (&!1 ⊔ &!0 ⊔ &!1 ⊔ &!0).
+    change_qual (openq (&!1 ⊔ &!0) &!1 (#!1 ⊔ &!0 ⊔ &!1 ⊔ &!0)).
+    change_type (open_ty TUnit ∅ (TRef ∅ TUnit) &!1 (TOPair (TRef ∅ ({TUnit | ∅} ==> {TUnit | ∅})) (TRef ∅ TUnit))).
+    2: unfold TOPair; ccrush.
+    apply t_app; try solve [ccrush].
+    * change_qual (openq (&!1 ⊔ &!0) &!0 (#!1 ⊔ &!1 ⊔ &!0)).
+      change_type (open_ty TUnit ∅ (TRef ∅ ({TUnit | ∅} ==> {TUnit | ∅})) &!0
+                           (({TRef ∅ TUnit | &! 1} ==> {TOPair (TRef ∅ ({TUnit | ∅} ==> {TUnit | ∅})) (TRef ∅ TUnit) | #!1 ⊔ #!3 ⊔ &!1 ⊔ &!0}))).
+      2 : { unfold TOPair; ccrush. f_equal. qdec. }
+      apply t_app; try solve [ccrush].
+      + apply t_pair_mk_inst.
+      + change_qual (∅ ⊔ &!0). apply t_loc; ccrush.
+      + ccrush. replace (qset false {}N {}N (union (singleton 1) (singleton 0))) with (&!1 ⊔ &!0). eauto using sat_loc_0, sat_loc_1. ccrush.
+    * change_qual (∅ ⊔ &!1). apply t_loc; ccrush.
+    * ccrush. replace (qset false {}N {}N (union (singleton 0) (union (singleton 1) (singleton 0)))) with (&!1 ⊔ &!0). eauto using sat_loc_0, sat_loc_1. ccrush.
+  Qed.
+
+  Example t_fst_pair_of_refs : has_type [] φ Σ fst_pair_of_refs (TRef ∅ ({TUnit | ∅} ==> {TUnit | ∅})) (&!0 ⊔ &!1).
+  Proof.
+    unfold fst_pair_of_refs.
+    change_qual (openq (&!0 ⊔ &!1) (&!1 ⊔ &!0) (&!0 ⊔ &!1)).
+    change_type (open_ty TUnit ∅ (TOPair (TRef ∅ ({TUnit | ∅} ==> {TUnit | ∅})) (TRef ∅ TUnit)) (&!1 ⊔ &!0) (TRef ∅ ({TUnit | ∅} ==> {TUnit | ∅}))).
+    apply t_app; try solve [ccrush].
+    * replace (&! 1 ⊔ &! 0) with (&!0 ⊔ &!1). apply t_fst_inst. ccrush.
+    * apply t_pair_of_refs.
+    * ccrush. ccrush. replace (qset false {}N {}N (union (singleton 0) (singleton 1))) with (&!0 ⊔ &!1). eauto using sat_loc_0, sat_loc_1. ccrush.
+  Qed.
+
+  Example t_snd_pair_of_refs : has_type [] φ Σ snd_pair_of_refs (TRef ∅ TUnit) (&!0 ⊔ &!1).
+  Proof.
+    unfold snd_pair_of_refs.
+    change_qual (openq (&!0 ⊔ &!1) (&!1 ⊔ &!0) (&!0 ⊔ &!1)).
+    change_type (open_ty TUnit ∅ (TOPair (TRef ∅ ({TUnit | ∅} ==> {TUnit | ∅})) (TRef ∅ TUnit)) (&!1 ⊔ &!0) (TRef ∅ TUnit)).
+    apply t_app; try solve [ccrush].
+    * replace (&! 1 ⊔ &! 0) with (&!0 ⊔ &!1). apply t_snd_inst. ccrush.
+    * apply t_pair_of_refs.
+    * ccrush. ccrush. replace (qset false {}N {}N (union (singleton 0) (singleton 1))) with (&!0 ⊔ &!1). eauto using sat_loc_0, sat_loc_1. ccrush.
+  Qed.
+
+End OpaquePairUse.
+
+Section OpaquePairEndToEnd.
+
+  (* Now we demonstrate the "counter" example (Fig. 1 of the paper). *)
+
+  Example TThunk := ({TUnit | ∅ } ==> {TUnit | ∅}).
+
+  (* def counter() =
+       let x = new Ref()
+       pair_mk({() => x:=!x}, {() => x:=!x})
+  *)
+  Example counter := (tabs (tlet (tref tunit)
+                                 (tapp (tapp (ttapp (ttapp pair_mk)) (tabs (tassign #3 (tderef #3))))
+                                                                     (tabs (tassign #3 (tderef #3)))))).
+
+  (* let ctr = counter()
+     let i = fst(ctr)
+     let d = fst(ctr)
+  *)
+  Example counter_use := (tlet (tapp counter tunit)
+                                (tlet (tapp (ttapp (ttapp fst)) #1)
+                                      (tapp (ttapp (ttapp snd)) #3))).
+
+
+  (* Type of the pair constructor instantation in its usage context within counter. The concrete typing assumptions
+     are unimportant and left abstract: *)
+  Example t_counter_pair_mk_inst : forall {W X Y Z},
+    has_type [bind_tm (false, W, {♦}); bind_tm (true, X, ∅); bind_tm (false, Y, ∅); bind_tm (true, Z, ∅)]
+             $♦3 [] (* <- we have access to the local mutable reference cell x, bound to $3 *)
+             (ttapp (ttapp pair_mk)) ({TThunk | $! 3} ==> {{TThunk | $! 3} ==> {TOPair TThunk TThunk | #! 1 ⊔ #! 3 ⊔ $! 3 ⊔ $! 3} | #! 1 ⊔ $! 3 ⊔ $! 3 }) $!3.
+  Proof.
+    intros. change_qual ($!3 ⊔ $!3).
+    change_qual (openq $!3 $!3 (#!1 ⊔ $!3)).
+    change_type (open_ty TUnit ∅ TThunk $!3 ({TThunk | $! 3} ==> {{#3 | #!3} ==> {TOPair TThunk #9 | #! 1 ⊔ #! 3 ⊔ #!5 ⊔ $! 3 } | #! 1 ⊔ #!3 ⊔ $! 3 })).
+    2: unfold TThunk; unfold TOPair; ccrush.
+    apply t_tapp_fresh with (d1':=$♦3) (df':=$♦3); try solve [unfold TThunk; ccrush].
+    dom_equals ($♦3). apply (t_sub_bound ⊤ $♦3); try solve [ccrush].
+    change_qual (openq ∅ $!3 #!1).
+    change_type (open_ty TUnit ∅ TThunk $!3 (∀<:{⊤ | #♦1}.{ {#3 | #!3} ==> {{# 3 | #! 3} ==> {TOPair #9 # 9 | #! 1 ⊔ #! 3 ⊔ #! 5 ⊔ #!7} | #! 1 ⊔ #!3 ⊔ #!5} | #! 1 ⊔ #! 3})).
+    2: unfold TThunk; unfold TOPair; ccrush.
+    apply t_tapp_fresh with (d1':=$♦3) (df':=∅); try solve [unfold TThunk; ccrush].
+    dom_equals ({♦}). apply (t_sub_bound ⊤ {♦}); try solve [ccrush].
+    apply t_pair_mk; ccrush.
+  Qed.
+
+  (* counter : Unit => OPair[Thunk,Thunk]^{♦} *)
+  Example t_counter : has_type [] ∅ [] counter ({TUnit | ∅ } ==> { (TOPair TThunk TThunk) | {♦} }) ∅.
+  Proof.
+    unfold counter.
+    apply t_abs; try solve [ccrush]. unfold TThunk; unfold TOPair; ccrush.
+    (* a little cleanup *)
+    unfold_open. repeat rewrite open_let. cleanup. fold pair_mk. fold TThunk.
+    replace (qset false {}N (union (singleton 3) (singleton 1)) {}N) with (#!3 ⊔ #!1); try solve [ccrush]. fold (TOPair TThunk TThunk).
+    (* prepare dependent application/let rule *)
+    change_qual (openq ∅ {♦} #!1).
+    change_type ((TOPair TThunk TThunk) <~ᵀ TUnit ~ ∅; (TRef ∅ TUnit) ~ {♦}). 2: unfold TThunk; unfold TOPair; ccrush.
+    apply t_let_fresh with (q1':={♦}) (df':=∅); ccrush. unfold TThunk; unfold TOPair. ccrush.
+    * (* binding *) change_qual (∅ ⊔ {♦}). apply t_ref; ccrush. apply t_base; ccrush.
+    * (* body *) fold pair_mk. fold TThunk.
+      replace (qset false {}N (union (singleton 3) (singleton 1)) {}N) with (#!3 ⊔ #!1); try solve [ccrush]. fold (TOPair TThunk TThunk).
+      change_qual (openq $!3 $!3 (#!1 ⊔ $!3)).
+      change_type ((TOPair TThunk TThunk) <~ᵀ TUnit ~ ∅; TThunk ~  $! 3). 2: unfold TThunk; unfold TOPair; ccrush.
+      apply t_app; try solve [ccrush].
+      + change_qual (openq $!3 $!3 (#!1 ⊔ $!3 ⊔ $!3)).
+        change_type (({TThunk | $! 3} ==> {TOPair TThunk TThunk | #!1 ⊔ #!3 ⊔ $!3 ⊔ $!3}) <~ᵀ TUnit ~ ∅; TThunk ~ $! 3).
+        2: { unfold TThunk; unfold TOPair; ccrush. f_equal. qdec. }
+        apply t_app; try solve [ccrush].
+        - (* constructor*)
+          apply t_counter_pair_mk_inst.
+        - (* thunk *) apply t_abs; ccrush.
+          eapply t_assign.
+          ** eapply t_var; ccrush.
+          ** eapply t_deref. eapply t_var; ccrush. all: ccrush.
+          ** auto.
+      + (* thunk *) apply t_abs; ccrush.
+        eapply t_assign.
+        ** eapply t_var; ccrush.
+        ** eapply t_deref. eapply t_var; ccrush. all: ccrush.
+        ** auto.
+  Qed.
+
+  (* Type of the first projection its usage context within counter_use. The concrete typing assumptions
+     are unimportant and left abstract:
+     fst: OPair[Thunk,Thunk]^ctr => Thunk^ctr
+     *)
+  Example t_counter_use_fst_inst : forall {X Y},
+    has_type [bind_tm (false, X, {♦}); bind_tm (true, Y, ∅)] $♦ 1 [] (ttapp (ttapp fst)) ({TOPair TThunk TThunk | $! 1} ==> {TThunk | $! 1 ⊔ $! 1}) $!1.
+  Proof.
+    intros. change_qual (openq $!1 $!1 (#!1 ⊔ $!1)).
+    change_type (open_ty TUnit ∅ TThunk $!1 ({TOPair TThunk #5 | #!1 ⊔ $! 1} ==> {TThunk | #!3 ⊔ $! 1})).
+    2: { unfold TThunk; unfold TOPair; ccrush. f_equal. qdec. }
+    apply t_tapp_fresh with (d1':=$♦1) (df':=$♦1); try solve [ccrush]. 2 : unfold TThunk; ccrush.
+    dom_equals ($♦1). apply (t_sub_bound ⊤ ($♦1)); try solve [ccrush].
+    change_qual (openq ∅ $!1 #!1).
+    change_type (open_ty TUnit ∅ TThunk $!1 (∀<:{⊤ | #♦ 1}.{ {TOPair #5 # 5 | #! 1 ⊔ #!3} ==> {#5| #! 3 ⊔ #!5} | #! 1 ⊔ #!3})).
+    2: unfold TThunk; unfold TOPair; ccrush.
+    apply t_tapp_fresh with (d1':=$♦1) (df':=∅); try solve [ccrush]. 2 : unfold TThunk; ccrush.
+    dom_equals ({♦}). apply (t_sub_bound ⊤ ({♦})); try solve [ccrush].
+    apply t_fst; ccrush.
+  Qed.
+
+  (* Type of the second projection its usage context within counter_use. The concrete typing assumptions
+     are unimportant and left abstract:
+     snd: OPair[Thunk,Thunk]^ctr => Thunk^ctr*)
+  Example t_counter_use_snd_inst : forall {W X Y Z},
+    has_type [bind_tm (false, W, $♦ 1); bind_tm (true, X, $! 1); bind_tm (false, Y, {♦}); bind_tm (true, Z, ∅)]
+             (qset true (union (singleton 1) (singleton 3)) {}N {}N) []
+             (ttapp (ttapp snd)) ({TOPair TThunk TThunk | $! 1} ==> {TThunk | $! 1 ⊔ $! 1}) $!1.
+  Proof.
+    intros. change_qual (openq $!1 $!1 (#!1 ⊔ $!1)).
+    change_type (open_ty TUnit ∅ TThunk $!1 ({TOPair TThunk #5 | #!1 ⊔ $! 1} ==> {#3 | #!3 ⊔ $! 1})).
+    2: { unfold TThunk; unfold TOPair; ccrush. f_equal. qdec. }
+    apply t_tapp_fresh with (d1':=$♦1) (df':=$♦1); try solve [ccrush]. 2 : unfold TThunk; ccrush.
+    dom_equals ($♦1). apply (t_sub_bound ⊤ ($♦1)); try solve [ccrush].
+    change_qual (openq ∅ $!1 #!1).
+    change_type (open_ty TUnit ∅ TThunk $!1 (∀<:{⊤ | #♦ 1}.{ {TOPair #5 # 5 | #! 1 ⊔ #!3} ==> {#3| #! 3 ⊔ #!5} | #! 1 ⊔ #!3})).
+    2: unfold TThunk; unfold TOPair; ccrush.
+    apply t_tapp_fresh with (d1':=$♦1) (df':=∅); try solve [ccrush]. 2 : unfold TThunk; ccrush.
+    dom_equals ({♦}). apply (t_sub_bound ⊤ ({♦})); try solve [ccrush].
+    apply t_snd; ccrush.
+  Qed.
+
+  (* counter_use : Thunk^{♦}*)
+  Example t_counter_use : has_type [] {♦} [] counter_use TThunk {♦}.
+  Proof.
+    unfold counter_use.
+    change_qual (openq ∅ {♦} #!1).
+    change_type (open_ty TUnit ∅ (TOPair TThunk TThunk) {♦} TThunk).
+    apply t_let_fresh with (q1':={♦}) (df':={♦}); try solve [ccrush]. 1 : unfold TOPair; unfold TThunk; ccrush.
+    * (* counter : OPair[Thunk,Thunk]^{♦} *) dep_app (∅) (∅). 2: unfold TOPair; unfold TThunk; ccrush.
+      apply t_app; try solve [ccrush].
+      eapply weaken_flt. apply t_counter. all: ccrush.
+    * cleanup. fold TThunk. fold fst. fold snd.
+      change_qual (openq $!1 $!1 $!1).
+      change_type (open_ty TUnit ∅ TThunk $!1 TThunk).
+      eapply t_let_fresh with (q1':=$♦1) (df':=$♦1); try solve [unfold TOPair; unfold TThunk; ccrush].
+      + (* fst(counter) : Thunk^{counter} *)
+        change_qual (openq $!1 $!1 ($!1 ⊔ $!1)).
+        change_type (open_ty TUnit ∅ (TOPair TThunk TThunk) $!1 TThunk).
+        apply t_app; try solve [ccrush].
+        - apply t_counter_use_fst_inst.
+        - eapply t_var; ccrush. unfold TOPair; unfold TThunk; ccrush.
+      + (* snd(counter) : Thunk^{counter} *)
+        cleanup. fold snd. fold TThunk.
+        change_qual (openq $!1 $!1 ($!1 ⊔ $!1)).
+        change_type (open_ty TUnit ∅ (TOPair TThunk TThunk) $!1 TThunk).
+        apply t_app; try solve [ccrush].
+        - apply t_counter_use_snd_inst.
+        - eapply t_var; ccrush. unfold TOPair; unfold TThunk; ccrush.
+  Qed.
+
+End OpaquePairEndToEnd.
+
+Section PairTransparentToOpaque.
+
+  (* Finally, we assert that transparent pairs are convertible into opaque pairs by typing an eta expansion.
+     If we take the Church encodings as a justification for data types, then we can use this eta expansion
+     as an admissible subtyping rule linking the two encodings. We can then use this thereby justified subtyping rule
+     for data types escaping their defining scope.
+
+     We believe that we can alternatively replace this justification by eta expansion with a pure subtyping argument
+     using self-type abstraction, which is yet to be mechanized.
+  *)
+
+  (* Convert a transparent pair to an opaque pair by eta expansion:
+     pair_to_opair = ΛA.ΛB.λp.pair_mk(fst(p),snd(p))
+  *)
+  Example pair_to_opair := (ttabs (ttabs (tabs (tapp (tapp (ttapp (ttapp pair_mk)) (tapp (ttapp (ttapp fst)) #1)) (tapp (ttapp (ttapp snd)) #1))))).
+
+  (* Instantiation of fst used in the function
+     fst: Pair[A^a,B^b]^{a,b} => A^a
+  *)
+  Lemma fst_pair_to_opair_inst: forall {X0 X1 X2 X3 X4 X5}, has_type
+      [bind_tm (false, X5, qset false (union (singleton 1) (singleton 3)) {}N {}N);
+       bind_tm (true,  X4, qset false (union (singleton 1) (singleton 3)) {}N {}N);
+       bind_ty (false, X3, $♦ 1);
+       bind_tm (true,  X2, $! 1);
+       bind_ty (false, X1, {♦});
+       bind_tm (true,  X0, ∅)]
+      (qset true (union (union (singleton 1) (singleton 3)) (union (singleton 4) (singleton 5))) {}N {}N)
+      [] (ttapp (ttapp fst)) ({TPair $ 1 $! 1 $! 1 $ 3 $! 3 $! 3 $! 3 | $! 1 ⊔ $! 3} ==> {$ 1 | $! 1})  ($! 1 ⊔ $! 3).
+  Proof.
+    intros.
+    apply t_sub with (T1:=({TPair $ 1 $! 1 $! 1 $ 3 $! 3 $! 3 $! 3 | $! 1 ⊔ $! 3 ⊔ {♦}} ==> {$ 1 | $! 1})) (d1:=($! 1 ⊔ $! 3)). 3,4 : ccrush.
+    * change_qual (openq $!1 $!3 (#!1 ⊔ $!1)).
+      change_type (open_ty TUnit ∅ $3 $!3
+                         ({TPair $ 1 $! 1 $! 1 #5 #!1 #!3 #!5 | #!1 ⊔ $! 1 ⊔ {♦}} ==> {$ 1 | $! 1})). 2: unfold TPair; ccrush.
+      apply t_tapp_fresh with (d1':=$♦3⊔$♦1) (df':=$♦1); try solve [ccrush].
+      - dom_equals ($♦1). apply (t_sub_bound ⊤ $♦1); try solve [ccrush].
+        change_qual (openq ∅ $!1 #!1).
+        change_type (open_ty TUnit ∅ $1 $!1
+             (∀<:{⊤ | #♦1}.{ {TPair #5 #!3 #!5 # 5 #! 1 #! 3 #! 5 | #! 1 ⊔ #!3 ⊔ {♦}} ==> {#5 | #!5} | #! 1 ⊔ #!3})).
+        2: unfold TPair; ccrush.
+        apply t_tapp_fresh with (d1':=$♦1) (df':=∅); try solve [ccrush].
+        dom_equals ({♦}). apply (t_sub_bound ⊤ {♦}); try solve [ccrush].
+        apply t_fst1; ccrush.
+      - (* show transitive reachability closure of this qualifier, could be further automated *)
+        constructor; eauto. unfold tenv_saturated. intros.
+        repeat rewrite qmem_lub_or_commute in H. destruct H as [ Hmem  | Hmem];
+        simpl in Hmem; apply NatSetFacts.singleton_iff in Hmem; subst;
+        try solve [eapply sat_tvar; ccrush]; try solve [eapply sat_var; ccrush].
+    * apply s_fun. 1,2: unfold TPair; ccrush.
+      apply qs_sq; ccrush.
+      apply stp_refl. unfold TPair; ccrush. apply qs_sq; ccrush.
+      cleanup. apply stp_refl; ccrush. apply qs_sq; ccrush.
+  Qed.
+
+  (* Instantiation of snd used in the function
+     snd: Pair[A^a,B^b]^{a,b} => B^b
+  *)
+  Lemma snd_pair_to_opair_inst: forall {X0 X1 X2 X3 X4 X5}, has_type
+      [bind_tm (false, X5, qset false (union (singleton 1) (singleton 3)) {}N {}N);
+       bind_tm (true,  X4, qset false (union (singleton 1) (singleton 3)) {}N {}N);
+       bind_ty (false, X3, $♦ 1);
+       bind_tm (true,  X2, $! 1);
+       bind_ty (false, X1, {♦});
+       bind_tm (true,  X0, ∅)]
+      (qset true (union (union (singleton 1) (singleton 3)) (union (singleton 4) (singleton 5))) {}N {}N)
+      [] (ttapp (ttapp snd)) ({TPair $ 1 $! 1 $! 1 $ 3 $! 3 $! 3 $! 3 | $! 1 ⊔ $! 3} ==> {$ 3 | $! 3})  ($! 1 ⊔ $! 3).
+  Proof.
+    intros.
+    apply t_sub with (T1:=({TPair $ 1 $! 1 $! 1 $ 3 $! 3 $! 3 $! 3 | $! 1 ⊔ $! 3 ⊔ {♦}} ==> {$ 3 | $! 3})) (d1:=($! 1 ⊔ $! 3)). 3,4 : ccrush.
+    * change_qual (openq $!1 $!3 (#!1 ⊔ $!1)).
+      change_type (open_ty TUnit ∅ $3 $!3
+                         ({TPair $ 1 $! 1 $! 1 #5 #!1 #!3 #!5 | #!1 ⊔ $! 1 ⊔ {♦}} ==> {#3 | #!3})). 2: unfold TPair; ccrush.
+      apply t_tapp_fresh with (d1':=$♦3⊔$♦1) (df':=$♦1); try solve [ccrush].
+      - dom_equals ($♦1). apply (t_sub_bound ⊤ $♦1); try solve [ccrush].
+        change_qual (openq ∅ $!1 #!1).
+        change_type (open_ty TUnit ∅ $1 $!1
+             (∀<:{⊤ | #♦1}.{ {TPair #5 #!3 #!5 # 5 #! 1 #! 3 #! 5 | #! 1 ⊔ #!3 ⊔ {♦}} ==> {#3 | #!3} | #! 1 ⊔ #!3})).
+        2: unfold TPair; ccrush.
+        apply t_tapp_fresh with (d1':=$♦1) (df':=∅); try solve [ccrush].
+        dom_equals ({♦}). apply (t_sub_bound ⊤ {♦}); try solve [ccrush].
+        apply t_snd1; ccrush.
+      - (* show transitive reachability closure of this qualifier, could be further automated *)
+        constructor; eauto. unfold tenv_saturated. intros.
+        repeat rewrite qmem_lub_or_commute in H. destruct H as [ Hmem  | Hmem];
+        simpl in Hmem; apply NatSetFacts.singleton_iff in Hmem; subst;
+        try solve [eapply sat_tvar; ccrush]; try solve [eapply sat_var; ccrush].
+    * apply s_fun. 1,2: unfold TPair; ccrush.
+      apply qs_sq; ccrush.
+      apply stp_refl. unfold TPair; ccrush. apply qs_sq; ccrush.
+      cleanup. apply stp_refl; ccrush. apply qs_sq; ccrush.
+  Qed.
+
+  (* The eta expansion is typable and justifies converting transparent pairs to opaque pairs:
+     pair_to_opair : (∀A^a<:⊤♦. (∀B^b<:⊤♦a. (Pair[A^a,B^b] => OPair[A,B]^{a,b})^{a,b})^{a})^∅
+   *)
+  Example t_pair_to_opair : has_type [] ∅ [] pair_to_opair (∀.{ ∀<:{ #♦1 }.{ { TPair #5 #!3 #!5 #5 #!1 #!3 #!5 | #!3 ⊔ #!1 } ==> {TOPair #7 #7 | #!3 ⊔ #!5} | #!1 ⊔ #!3  } | #!1 }) ∅.
+  Proof.
+    unfold pair_to_opair.
+    apply t_tabs; ccrush. (* 0/1 <- A^a *)
+    unfold TPair; unfold TOPair; ccrush.
+    apply t_tabs; ccrush. (* 2/3 <- B^b *)
+    apply t_abs; ccrush.  (* 4/5 <- p *)
+    (* a little cleanup *)
+    fold pair_mk. fold fst. fold snd.
+    change_type (TOPair $1 $3). 2: unfold TOPair; ccrush.
+    change_qual (openq ($!1 ⊔ $!3 ⊔ $!1) $!3  (#!1 ⊔ $!1 ⊔ $!3 ⊔ $!1)).
+    change_type (open_ty TUnit ∅ $3 $!3 (TOPair $1 $3)). 2 : unfold TOPair; ccrush.
+    apply t_app; try solve [ccrush].
+    * change_qual (openq ($!3 ⊔ $!1) $!1 (#!1 ⊔ $!3 ⊔ $!1)).
+      change_type (open_ty TUnit ∅ $1 $!1
+      ({$ 3 | $! 3} ==> {TOPair $1 $3 | #! 1 ⊔ #!3 ⊔ $! 3 ⊔ $! 1})).
+      2 : { unfold TOPair; ccrush. f_equal. qdec. }
+      apply t_app; try solve [ccrush].
+      + change_qual (openq $!1 $!3 (#!1 ⊔ $!1)).
+        change_type (open_ty TUnit ∅ $3 $!3 ({$ 1 | $! 1}
+                                           ==> {{#3| #!3}
+                                                     ==> {TOPair $1 #9 | #! 1 ⊔ #! 3 ⊔ #!5 ⊔ $! 1} | #! 1 ⊔ #! 3 ⊔ $! 1})).
+        2 : { unfold TOPair; ccrush. f_equal. qdec. f_equal. qdec. }
+        apply t_tapp_fresh with (d1':=$♦3⊔$♦1) (df':=$♦1); try solve [ccrush].
+        - dom_equals ($♦1). apply (t_sub_bound ⊤ $♦1); try solve [ccrush].
+          change_qual (openq ∅ $!1 #!1).
+          change_type (open_ty TUnit ∅ $1 $!1 (∀<:{⊤ | #♦1}.{
+            {#3| #!3}
+               ==> {{# 3 | #! 3}
+                       ==> {TOPair #9 #9
+                           | #! 1 ⊔ #! 3 ⊔ #! 5 ⊔ #!7}
+                   | #! 1 ⊔ #! 3 ⊔ #!5}
+            | #! 1 ⊔ #!3})).
+          2 : unfold TOPair; ccrush.
+          apply t_tapp_fresh with (d1':=$♦1) (df':=∅); try solve [ccrush].
+          dom_equals ({♦}).  apply (t_sub_bound ⊤ {♦}); try solve [ccrush].
+          apply t_pair_mk; ccrush.
+        - (* show transitive reachability closure of this qualifier, could be further automated *)
+          constructor; eauto. unfold tenv_saturated. intros.
+          repeat rewrite qmem_lub_or_commute in H. destruct H as [ Hmem  | Hmem];
+          simpl in Hmem; apply NatSetFacts.singleton_iff in Hmem; subst;
+          try solve [eapply sat_tvar; ccrush]; try solve [eapply sat_var; ccrush].
+      + (* fst p*)
+        change_qual (openq ($!1 ⊔ $!3) ($!1 ⊔ $!3) $!1).
+        change_type (open_ty TUnit ∅ (TPair $1 $!1 $!1 $3 $!3 $!3 $!3) ($!1 ⊔ $!3) $1).
+        apply t_app; try solve [ccrush].
+        - apply fst_pair_to_opair_inst.
+        - eapply t_sub.
+          eapply t_var; ccrush. 2-3 : ccrush.
+          unfold TPair. cleanup. apply stp_refl; ccrush.
+          eapply qs_qvar; ccrush.
+    * (* snd p*)
+      change_qual (openq ($!1 ⊔ $!3) ($!1 ⊔ $!3) $!3).
+      change_type (open_ty TUnit ∅ (TPair $1 $!1 $!1 $3 $!3 $!3 $!3) ($!1 ⊔ $!3) $3).
+      apply t_app; try solve [ccrush].
+      - apply snd_pair_to_opair_inst.
+      - eapply t_sub.
+        eapply t_var; ccrush. 2-3 : ccrush.
+        unfold TPair. cleanup. apply stp_refl; ccrush.
+        eapply qs_qvar; ccrush.
+    Qed.
+
+End PairTransparentToOpaque.
